<?xml version="1.0"?>
<rdf:RDF xmlns="http://purl.org/poso/"
     xml:base="http://purl.org/poso/"
     xmlns:owl="http://www.w3.org/2002/07/owl#"
     xmlns:rdf="http://www.w3.org/1999/02/22-rdf-syntax-ns#"
     xmlns:xml="http://www.w3.org/XML/1998/namespace"
     xmlns:xsd="http://www.w3.org/2001/XMLSchema#"
     xmlns:foaf="http://xmlns.com/foaf/0.1/"
     xmlns:qudt="http://qudt.org/schema/qudt/"
     xmlns:rdfs="http://www.w3.org/2000/01/rdf-schema#"
     xmlns:skos="http://www.w3.org/2004/02/skos/core#"
     xmlns:vann="http://purl.org/vocab/vann/"
     xmlns:terms="http://purl.org/dc/terms/"
     xmlns:schema="http://schema.org/">
    <owl:Ontology rdf:about="http://purl.org/poso/">
        <owl:versionIRI rdf:resource="http://purl.org/poso/1.0/"/>
        <owl:imports rdf:resource="http://www.w3.org/ns/ssn/"/>
        <owl:imports rdf:resource="http://www.w3.org/ns/ssn/systems/"/>
        <terms:abstract xml:lang="en">The positioning system ontology is a vocabulary for describing positioning systems and the techniques these systems use to determine a position. With POSO we aim to provide semantic meaning on how a positioning system is deployed and how results are calculated.</terms:abstract>
        <terms:bibliographicCitation>Maxim Van de Wynckel and Beat Signer, POSO: A Generic Positioning System Ontology</terms:bibliographicCitation>
        <terms:contributor xml:lang="en">Beat Signer</terms:contributor>
        <terms:creator xml:lang="en">Maxim Van de Wynckel</terms:creator>
        <terms:description>This ontology provides the terminologies used for positioning systems.</terms:description>
        <terms:license rdf:resource="http://purl.org/NET/rdflicense/MIT1.0"/>
        <terms:modified rdf:datatype="http://www.w3.org/2001/XMLSchema#dateTime">2023-01-26T00:00:00</terms:modified>
        <terms:title xml:lang="en">Positioning System Ontology</terms:title>
        <vann:preferredNamespacePrefix>poso</vann:preferredNamespacePrefix>
        <vann:preferredNamespaceUri rdf:datatype="http://www.w3.org/2001/XMLSchema#anyURI">http://purl.org/poso/</vann:preferredNamespaceUri>
        <schema:image>https://raw.githubusercontent.com/OpenHPS/POSO/main/docs/images/systems_and_procedures.svg</schema:image>
    </owl:Ontology>
    


    <!-- 
    ///////////////////////////////////////////////////////////////////////////////////////
    //
    // Annotation properties
    //
    ///////////////////////////////////////////////////////////////////////////////////////
     -->


    


    <!-- http://purl.org/dc/terms/abstract -->


    <owl:AnnotationProperty rdf:about="http://purl.org/dc/terms/abstract"/>
    


    <!-- http://purl.org/dc/terms/bibliographicCitation -->


    <owl:AnnotationProperty rdf:about="http://purl.org/dc/terms/bibliographicCitation"/>
    


    <!-- http://purl.org/dc/terms/contributor -->


    <owl:AnnotationProperty rdf:about="http://purl.org/dc/terms/contributor"/>
    


    <!-- http://purl.org/dc/terms/creator -->


    <owl:AnnotationProperty rdf:about="http://purl.org/dc/terms/creator"/>
    


    <!-- http://purl.org/dc/terms/description -->


    <owl:AnnotationProperty rdf:about="http://purl.org/dc/terms/description"/>
    


    <!-- http://purl.org/dc/terms/license -->


    <owl:AnnotationProperty rdf:about="http://purl.org/dc/terms/license"/>
    


    <!-- http://purl.org/dc/terms/modified -->


    <owl:AnnotationProperty rdf:about="http://purl.org/dc/terms/modified"/>
    


    <!-- http://purl.org/dc/terms/source -->


    <owl:AnnotationProperty rdf:about="http://purl.org/dc/terms/source"/>
    


    <!-- http://purl.org/dc/terms/title -->


    <owl:AnnotationProperty rdf:about="http://purl.org/dc/terms/title"/>
    


    <!-- http://purl.org/vocab/vann/preferredNamespacePrefix -->


    <owl:AnnotationProperty rdf:about="http://purl.org/vocab/vann/preferredNamespacePrefix"/>
    


    <!-- http://purl.org/vocab/vann/preferredNamespaceUri -->


    <owl:AnnotationProperty rdf:about="http://purl.org/vocab/vann/preferredNamespaceUri"/>
    


    <!-- http://qudt.org/schema/qudt/example -->


    <owl:AnnotationProperty rdf:about="http://qudt.org/schema/qudt/example"/>
    


    <!-- http://qudt.org/schema/qudt/hasQuantityKind -->


    <owl:AnnotationProperty rdf:about="http://qudt.org/schema/qudt/hasQuantityKind"/>
    


    <!-- http://schema.org/image -->


    <owl:AnnotationProperty rdf:about="http://schema.org/image"/>
    


    <!-- http://www.w3.org/2004/02/skos/core#altLabel -->


    <owl:AnnotationProperty rdf:about="http://www.w3.org/2004/02/skos/core#altLabel"/>
    


    <!-- 
    ///////////////////////////////////////////////////////////////////////////////////////
    //
    // Object Properties
    //
    ///////////////////////////////////////////////////////////////////////////////////////
     -->


    


    <!-- http://purl.org/poso/angle -->


    <owl:ObjectProperty rdf:about="http://purl.org/poso/angle">
        <rdf:type rdf:resource="http://www.w3.org/2002/07/owl#FunctionalProperty"/>
        <rdfs:domain rdf:resource="http://www.w3.org/ns/sosa/Result"/>
        <rdfs:range rdf:resource="http://www.w3.org/2000/01/rdf-schema#Class"/>
        <rdfs:comment xml:lang="en">Quantitative anglue result value for axis-angle representation.</rdfs:comment>
        <rdfs:label xml:lang="en">angle</rdfs:label>
        <rdfs:label xml:lang="nl">hoek</rdfs:label>
    </owl:ObjectProperty>
    


    <!-- http://purl.org/poso/hasAcceleration -->


    <owl:ObjectProperty rdf:about="http://purl.org/poso/hasAcceleration">
        <rdfs:subPropertyOf rdf:resource="http://www.w3.org/ns/ssn/hasProperty"/>
        <owl:inverseOf rdf:resource="http://purl.org/poso/isAccelerationOf"/>
        <rdfs:domain rdf:resource="http://www.w3.org/ns/sosa/FeatureOfInterest"/>
        <rdfs:range rdf:resource="http://purl.org/poso/Acceleration"/>
        <rdfs:comment xml:lang="en">Property that links a feature of interest to a unique acceleration property related to this feature.</rdfs:comment>
        <rdfs:label xml:lang="en">has acceleration</rdfs:label>
        <rdfs:label xml:lang="nl">heeft versnelling</rdfs:label>
    </owl:ObjectProperty>
    


    <!-- http://purl.org/poso/hasAccuracy -->


    <owl:ObjectProperty rdf:about="http://purl.org/poso/hasAccuracy">
        <rdfs:subPropertyOf rdf:resource="http://www.w3.org/ns/ssn/hasProperty"/>
        <rdf:type rdf:resource="http://www.w3.org/2002/07/owl#FunctionalProperty"/>
        <rdfs:comment xml:lang="en">The accuracy of an entity.</rdfs:comment>
        <rdfs:label xml:lang="en">has accuracy</rdfs:label>
        <rdfs:label xml:lang="nl">heeft accuraatheid</rdfs:label>
    </owl:ObjectProperty>
    


    <!-- http://purl.org/poso/hasCRS -->


    <owl:ObjectProperty rdf:about="http://purl.org/poso/hasCRS">
        <rdfs:subPropertyOf rdf:resource="http://purl.org/poso/hasSRS"/>
        <rdfs:label xml:lang="en">has coordinate reference system</rdfs:label>
        <rdfs:label xml:lang="nl">heeft een co√∂rdinaten referentiesysteem</rdfs:label>
    </owl:ObjectProperty>
    


    <!-- http://purl.org/poso/hasOrientation -->


    <owl:ObjectProperty rdf:about="http://purl.org/poso/hasOrientation">
        <rdfs:subPropertyOf rdf:resource="http://www.w3.org/ns/ssn/hasProperty"/>
        <owl:inverseOf rdf:resource="http://purl.org/poso/isOrientationOf"/>
        <rdfs:domain rdf:resource="http://www.w3.org/ns/sosa/FeatureOfInterest"/>
        <rdfs:range rdf:resource="http://purl.org/poso/Orientation"/>
        <rdfs:comment xml:lang="nl">Duid de orientatie aan van een object aan.</rdfs:comment>
        <rdfs:comment xml:lang="en">Indicates the orientation of a feature of interest.</rdfs:comment>
        <rdfs:label xml:lang="en">has orientation</rdfs:label>
        <rdfs:label xml:lang="nl">heeft orientatie</rdfs:label>
    </owl:ObjectProperty>
    


    <!-- http://purl.org/poso/hasPosition -->


    <owl:ObjectProperty rdf:about="http://purl.org/poso/hasPosition">
        <rdfs:subPropertyOf rdf:resource="http://www.w3.org/ns/ssn/hasProperty"/>
        <owl:inverseOf rdf:resource="http://purl.org/poso/isPositionOf"/>
        <rdfs:domain rdf:resource="http://www.w3.org/ns/sosa/FeatureOfInterest"/>
        <rdfs:range rdf:resource="http://purl.org/poso/Position"/>
        <rdfs:comment xml:lang="nl">Duid de absolute of relatieve positie van een object aan.</rdfs:comment>
        <rdfs:comment xml:lang="en">Indicates the absolute or relative position of a feature of interest.</rdfs:comment>
        <rdfs:label xml:lang="en">has position</rdfs:label>
        <rdfs:label xml:lang="nl">heeft positie</rdfs:label>
    </owl:ObjectProperty>
    


    <!-- http://purl.org/poso/hasRelativePosition -->


    <owl:ObjectProperty rdf:about="http://purl.org/poso/hasRelativePosition">
        <rdfs:subPropertyOf rdf:resource="http://purl.org/poso/hasPosition"/>
        <owl:inverseOf rdf:resource="http://purl.org/poso/isRelativeTo"/>
        <rdfs:range rdf:resource="http://purl.org/poso/RelativePosition"/>
        <rdfs:label xml:lang="en">has relative position</rdfs:label>
        <rdfs:label xml:lang="nl">heeft relatieve positie</rdfs:label>
    </owl:ObjectProperty>
    


    <!-- http://purl.org/poso/hasSRS -->


    <owl:ObjectProperty rdf:about="http://purl.org/poso/hasSRS">
        <rdfs:domain rdf:resource="http://www.w3.org/2002/07/owl#Thing"/>
        <qudt:example rdf:resource="http://www.opengis.net/def/crs/OGC/1.3/CRS84"/>
        <rdfs:comment xml:lang="en">Identifies an entity that has a spatial reference system in order to interpret the result.</rdfs:comment>
        <rdfs:label xml:lang="en">has spatial reference system</rdfs:label>
        <rdfs:label xml:lang="nl">heeft een ruimtelijk referentiepunt</rdfs:label>
    </owl:ObjectProperty>
    


    <!-- http://purl.org/poso/hasVelocity -->


    <owl:ObjectProperty rdf:about="http://purl.org/poso/hasVelocity">
        <rdfs:subPropertyOf rdf:resource="http://www.w3.org/ns/ssn/hasProperty"/>
        <owl:inverseOf rdf:resource="http://purl.org/poso/isVelocityOf"/>
        <rdfs:domain rdf:resource="http://www.w3.org/ns/sosa/FeatureOfInterest"/>
        <rdfs:range rdf:resource="http://purl.org/poso/Velocity"/>
        <rdfs:comment xml:lang="nl">Duid de snelheid van een object aan.</rdfs:comment>
        <rdfs:comment xml:lang="en">Indicates the velocity of a feature of interest.</rdfs:comment>
        <rdfs:label xml:lang="en">has velocity</rdfs:label>
        <rdfs:label xml:lang="nl">heeft snelheid</rdfs:label>
    </owl:ObjectProperty>
    


    <!-- http://purl.org/poso/inDeployment -->


    <owl:ObjectProperty rdf:about="http://purl.org/poso/inDeployment">
        <rdfs:domain rdf:resource="http://purl.org/poso/AbsolutePosition"/>
        <rdfs:range rdf:resource="http://www.w3.org/ns/ssn/Deployment"/>
        <vann:preferredNamespaceUri xml:lang="en">Identifies an absolute position within a deployment</vann:preferredNamespaceUri>
        <rdfs:label xml:lang="en">in deployment</rdfs:label>
    </owl:ObjectProperty>
    


    <!-- http://purl.org/poso/isAccelerationOf -->


    <owl:ObjectProperty rdf:about="http://purl.org/poso/isAccelerationOf">
        <rdfs:subPropertyOf rdf:resource="http://www.w3.org/ns/ssn/isPropertyOf"/>
        <rdfs:label xml:lang="en">is acceleration of</rdfs:label>
        <rdfs:label xml:lang="nl">is versnelling van</rdfs:label>
    </owl:ObjectProperty>
    


    <!-- http://purl.org/poso/isOrientationOf -->


    <owl:ObjectProperty rdf:about="http://purl.org/poso/isOrientationOf">
        <rdfs:subPropertyOf rdf:resource="http://www.w3.org/ns/ssn/isPropertyOf"/>
        <rdfs:label xml:lang="nl">is orientatie van</rdfs:label>
        <rdfs:label xml:lang="en">is orientation of</rdfs:label>
    </owl:ObjectProperty>
    


    <!-- http://purl.org/poso/isPositionOf -->


    <owl:ObjectProperty rdf:about="http://purl.org/poso/isPositionOf">
        <rdfs:subPropertyOf rdf:resource="http://www.w3.org/ns/ssn/isPropertyOf"/>
        <rdfs:label xml:lang="nl">is positie van</rdfs:label>
        <rdfs:label xml:lang="en">is position of</rdfs:label>
    </owl:ObjectProperty>
    


    <!-- http://purl.org/poso/isRelativeTo -->


    <owl:ObjectProperty rdf:about="http://purl.org/poso/isRelativeTo">
        <rdfs:domain rdf:resource="http://purl.org/poso/RelativePosition"/>
        <rdfs:range rdf:resource="http://www.w3.org/ns/sosa/FeatureOfInterest"/>
        <rdfs:comment xml:lang="en">Indicates a relative position to be relative to another feature of interest.</rdfs:comment>
        <rdfs:label xml:lang="nl">is relatief met</rdfs:label>
        <rdfs:label xml:lang="en">is relative to</rdfs:label>
        <skos:example xml:lang="en">A person can have a relative distance to another feature of interest. When a feature is moving (i.e. when the geometry changes based on time) the distance remains relative to the feature and not the geometry at a specific point in time.</skos:example>
    </owl:ObjectProperty>
    


    <!-- http://purl.org/poso/isVelocityOf -->


    <owl:ObjectProperty rdf:about="http://purl.org/poso/isVelocityOf">
        <rdfs:subPropertyOf rdf:resource="http://www.w3.org/ns/ssn/isPropertyOf"/>
        <rdfs:label xml:lang="nl">is de snelheid van</rdfs:label>
        <rdfs:label xml:lang="en">is velocity of</rdfs:label>
    </owl:ObjectProperty>
    


    <!-- http://purl.org/poso/madeBySystem -->


    <owl:ObjectProperty rdf:about="http://purl.org/poso/madeBySystem">
        <rdfs:domain rdf:resource="http://www.w3.org/ns/sosa/Observation"/>
        <rdfs:range rdf:resource="http://www.w3.org/ns/ssn/System"/>
        <rdfs:comment xml:lang="en">A relation to a re-usable system that computed the observation.</rdfs:comment>
        <rdfs:label xml:lang="nl">gemaakt door systeem</rdfs:label>
        <rdfs:label xml:lang="en">made by system</rdfs:label>
    </owl:ObjectProperty>
    


    <!-- http://purl.org/poso/observesType -->


    <owl:ObjectProperty rdf:about="http://purl.org/poso/observesType">
        <rdfs:subPropertyOf rdf:resource="http://www.w3.org/ns/ssn/forProperty"/>
        <rdfs:domain rdf:resource="http://www.w3.org/ns/ssn/System"/>
        <rdfs:range rdf:resource="http://www.w3.org/2000/01/rdf-schema#Class"/>
        <rdfs:comment xml:lang="en">The relation between a system and an observable property class to identify that a system observes a specific type of property.</rdfs:comment>
        <rdfs:label xml:lang="nl">observeert type</rdfs:label>
        <rdfs:label xml:lang="en">observes type</rdfs:label>
    </owl:ObjectProperty>
    


    <!-- http://purl.org/poso/pitch -->


    <owl:ObjectProperty rdf:about="http://purl.org/poso/pitch">
        <rdf:type rdf:resource="http://www.w3.org/2002/07/owl#FunctionalProperty"/>
        <rdfs:domain rdf:resource="http://purl.org/poso/EulerOrientation"/>
        <rdfs:range rdf:resource="http://www.w3.org/2000/01/rdf-schema#Class"/>
        <rdfs:comment xml:lang="en">Pitch is the rotation around the x-axis with respect to the object the yaw applies to.</rdfs:comment>
        <rdfs:label xml:lang="en">pitch</rdfs:label>
    </owl:ObjectProperty>
    


    <!-- http://purl.org/poso/roll -->


    <owl:ObjectProperty rdf:about="http://purl.org/poso/roll">
        <rdf:type rdf:resource="http://www.w3.org/2002/07/owl#FunctionalProperty"/>
        <rdfs:domain rdf:resource="http://purl.org/poso/EulerOrientation"/>
        <rdfs:range rdf:resource="http://www.w3.org/2000/01/rdf-schema#Class"/>
        <rdfs:comment xml:lang="en">Roll is the rotation around the y-axis with respect to the object the roll applies to.</rdfs:comment>
        <rdfs:label xml:lang="en">roll</rdfs:label>
    </owl:ObjectProperty>
    


    <!-- http://purl.org/poso/scalar -->


    <owl:ObjectProperty rdf:about="http://purl.org/poso/scalar">
        <rdf:type rdf:resource="http://www.w3.org/2002/07/owl#FunctionalProperty"/>
        <rdfs:domain rdf:resource="http://www.w3.org/ns/sosa/Result"/>
        <rdfs:range rdf:resource="http://www.w3.org/2000/01/rdf-schema#Class"/>
        <rdfs:label xml:lang="en">scalar</rdfs:label>
        <skos:altLabel>w</skos:altLabel>
    </owl:ObjectProperty>
    


    <!-- http://purl.org/poso/xAxisValue -->


    <owl:ObjectProperty rdf:about="http://purl.org/poso/xAxisValue">
        <rdf:type rdf:resource="http://www.w3.org/2002/07/owl#FunctionalProperty"/>
        <rdfs:domain rdf:resource="http://www.w3.org/ns/sosa/Result"/>
        <rdfs:range rdf:resource="http://www.w3.org/2000/01/rdf-schema#Class"/>
        <rdfs:comment xml:lang="en">Quantitative result value along the X-axis of a spatial sensor or result.</rdfs:comment>
        <rdfs:label xml:lang="en">x-axis value</rdfs:label>
    </owl:ObjectProperty>
    


    <!-- http://purl.org/poso/yAxisValue -->


    <owl:ObjectProperty rdf:about="http://purl.org/poso/yAxisValue">
        <rdf:type rdf:resource="http://www.w3.org/2002/07/owl#FunctionalProperty"/>
        <rdfs:domain rdf:resource="http://www.w3.org/ns/sosa/Result"/>
        <rdfs:range rdf:resource="http://www.w3.org/2000/01/rdf-schema#Class"/>
        <rdfs:comment xml:lang="en">Quantitative result value along the Y-axis of a spatial sensor or result.</rdfs:comment>
        <rdfs:label xml:lang="en">y-axis value</rdfs:label>
    </owl:ObjectProperty>
    


    <!-- http://purl.org/poso/yaw -->


    <owl:ObjectProperty rdf:about="http://purl.org/poso/yaw">
        <rdf:type rdf:resource="http://www.w3.org/2002/07/owl#FunctionalProperty"/>
        <rdfs:domain rdf:resource="http://purl.org/poso/EulerOrientation"/>
        <rdfs:range rdf:resource="http://www.w3.org/2000/01/rdf-schema#Class"/>
        <rdfs:comment xml:lang="en">Yaw is the rotation around the z-axis with respect to the object the yaw applies to.</rdfs:comment>
        <rdfs:label xml:lang="en">yaw</rdfs:label>
    </owl:ObjectProperty>
    


    <!-- http://purl.org/poso/zAxisValue -->


    <owl:ObjectProperty rdf:about="http://purl.org/poso/zAxisValue">
        <rdf:type rdf:resource="http://www.w3.org/2002/07/owl#FunctionalProperty"/>
        <rdfs:domain rdf:resource="http://www.w3.org/ns/sosa/Result"/>
        <rdfs:range rdf:resource="http://www.w3.org/2000/01/rdf-schema#Class"/>
        <rdfs:comment xml:lang="en">Quantitative result value along the Z-axis of a spatial sensor.</rdfs:comment>
        <rdfs:label xml:lang="en">z-axis value</rdfs:label>
    </owl:ObjectProperty>
    


    <!-- 
    ///////////////////////////////////////////////////////////////////////////////////////
    //
    // Classes
    //
    ///////////////////////////////////////////////////////////////////////////////////////
     -->


    


    <!-- http://purl.org/poso/AbsolutePosition -->


    <owl:Class rdf:about="http://purl.org/poso/AbsolutePosition">
        <owl:equivalentClass rdf:resource="http://www.opengis.net/ont/geosparql#Geometry"/>
        <rdfs:subClassOf rdf:resource="http://purl.org/poso/Position"/>
        <rdfs:comment xml:lang="en">An absolute position describes the position of an entity based on a fixed point in space. Usually this space is the Earth and the position is expressed in latitude and longitude.</rdfs:comment>
        <rdfs:label xml:lang="en">Absolute position</rdfs:label>
    </owl:Class>
    


    <!-- http://purl.org/poso/Acceleration -->


    <owl:Class rdf:about="http://purl.org/poso/Acceleration">
        <rdfs:subClassOf rdf:resource="http://www.w3.org/ns/sosa/ObservableProperty"/>
        <rdfs:subClassOf rdf:resource="http://www.w3.org/ns/sosa/Result"/>
        <qudt:hasQuantityKind rdf:resource="http://qudt.org/vocab/quantitykind/Acceleration"/>
        <rdfs:comment xml:lang="en">Acceleration is the (instantaneous) rate of change of velocity.</rdfs:comment>
        <rdfs:label xml:lang="en">Acceleration</rdfs:label>
        <rdfs:label xml:lang="nl">Versnelling</rdfs:label>
    </owl:Class>
    


    <!-- http://purl.org/poso/AngularAcceleration -->


    <owl:Class rdf:about="http://purl.org/poso/AngularAcceleration">
        <rdfs:subClassOf rdf:resource="http://purl.org/poso/Acceleration"/>
        <qudt:hasQuantityKind rdf:resource="http://qudt.org/vocab/quantitykind/AngularAcceleration"/>
        <rdfs:label xml:lang="en">Angular acceleration</rdfs:label>
        <rdfs:label xml:lang="nl">Draaiversnelling</rdfs:label>
    </owl:Class>
    


    <!-- http://purl.org/poso/AngularMovement -->


    <owl:Class rdf:about="http://purl.org/poso/AngularMovement">
        <rdfs:subClassOf rdf:resource="http://purl.org/poso/Movement"/>
        <rdfs:comment xml:lang="en">Angular movement around a certain origin point.</rdfs:comment>
        <rdfs:label xml:lang="en">Angular movement</rdfs:label>
        <rdfs:label xml:lang="nl">Draaibeweging</rdfs:label>
    </owl:Class>
    


    <!-- http://purl.org/poso/AngularVelocity -->


    <owl:Class rdf:about="http://purl.org/poso/AngularVelocity">
        <rdfs:subClassOf rdf:resource="http://purl.org/poso/Velocity"/>
        <qudt:hasQuantityKind rdf:resource="http://qudt.org/vocab/quantitykind/AngularVelocity"/>
        <rdfs:comment xml:lang="en">Angular velocity is the momentum around a point of origin.</rdfs:comment>
        <rdfs:label xml:lang="en">Angular velocity</rdfs:label>
        <rdfs:label xml:lang="nl">Draaisnelheid</rdfs:label>
    </owl:Class>
    


    <!-- http://purl.org/poso/Angulation -->


    <owl:Class rdf:about="http://purl.org/poso/Angulation">
        <rdfs:subClassOf rdf:resource="http://purl.org/poso/Triangulation"/>
        <rdfs:comment xml:lang="en">Angulation is a triangulation method to determine a position based on the relative angles to other objects.</rdfs:comment>
        <rdfs:label xml:lang="en">Angulation</rdfs:label>
    </owl:Class>
    


    <!-- http://purl.org/poso/AuditoryLandmark -->


    <owl:Class rdf:about="http://purl.org/poso/AuditoryLandmark">
        <rdfs:subClassOf rdf:resource="http://purl.org/poso/Landmark"/>
        <rdfs:comment xml:lang="en">A spatial landmark that can be observed by sound.</rdfs:comment>
        <rdfs:label xml:lang="en">Auditory landmark</rdfs:label>
    </owl:Class>
    


    <!-- http://purl.org/poso/AxisAngleOrientation -->


    <owl:Class rdf:about="http://purl.org/poso/AxisAngleOrientation">
        <rdfs:subClassOf rdf:resource="http://purl.org/poso/Orientation"/>
        <rdfs:subClassOf>
            <owl:Restriction>
                <owl:onProperty rdf:resource="http://purl.org/poso/angle"/>
                <owl:minCardinality rdf:datatype="http://www.w3.org/2001/XMLSchema#nonNegativeInteger">1</owl:minCardinality>
            </owl:Restriction>
        </rdfs:subClassOf>
        <rdfs:subClassOf>
            <owl:Restriction>
                <owl:onProperty rdf:resource="http://purl.org/poso/angle"/>
                <owl:maxCardinality rdf:datatype="http://www.w3.org/2001/XMLSchema#nonNegativeInteger">1</owl:maxCardinality>
            </owl:Restriction>
        </rdfs:subClassOf>
        <rdfs:subClassOf>
            <owl:Restriction>
                <owl:onProperty rdf:resource="http://purl.org/poso/xAxisValue"/>
                <owl:maxCardinality rdf:datatype="http://www.w3.org/2001/XMLSchema#nonNegativeInteger">1</owl:maxCardinality>
            </owl:Restriction>
        </rdfs:subClassOf>
        <rdfs:subClassOf>
            <owl:Restriction>
                <owl:onProperty rdf:resource="http://purl.org/poso/yAxisValue"/>
                <owl:maxCardinality rdf:datatype="http://www.w3.org/2001/XMLSchema#nonNegativeInteger">1</owl:maxCardinality>
            </owl:Restriction>
        </rdfs:subClassOf>
        <rdfs:subClassOf>
            <owl:Restriction>
                <owl:onProperty rdf:resource="http://purl.org/poso/zAxisValue"/>
                <owl:maxCardinality rdf:datatype="http://www.w3.org/2001/XMLSchema#nonNegativeInteger">1</owl:maxCardinality>
            </owl:Restriction>
        </rdfs:subClassOf>
        <rdfs:comment xml:lang="en">The axis-angle orientation is an orientation representation where the x, y and z values are rotated with a certain angle.</rdfs:comment>
        <rdfs:label xml:lang="en">Axis-angle orientation</rdfs:label>
    </owl:Class>
    


    <!-- http://purl.org/poso/BluetoothBeacon -->


    <owl:Class rdf:about="http://purl.org/poso/BluetoothBeacon">
        <rdfs:subClassOf rdf:resource="http://purl.org/poso/RFLandmark"/>
        <rdfs:comment xml:lang="en">A Bluetooth beacon is an RF landmark that advertises its transmission power and other optional information. Based on the signal strength receivers of this advertisement can determine the approximate distance.</rdfs:comment>
        <rdfs:label xml:lang="en">Bluetooth beacon</rdfs:label>
    </owl:Class>
    


    <!-- http://purl.org/poso/CellIdentification -->


    <owl:Class rdf:about="http://purl.org/poso/CellIdentification">
        <rdfs:subClassOf rdf:resource="http://purl.org/poso/PositioningTechnique"/>
        <rdfs:comment xml:lang="en">Cell identification is a positioning procedure using the position of one landmark that is within the cell.</rdfs:comment>
        <rdfs:label xml:lang="en">Cell identification</rdfs:label>
        <skos:altLabel xml:lang="en">Cell Of Origin (COO)</skos:altLabel>
        <skos:example xml:lang="en">An example of cell identification is using the position of a Bluetooth beacon whenever this beacon has a high signal strength.</skos:example>
        <skos:example xml:lang="en">An example of cell identification is using the position of a QR-code when this code is scanned (and the user is presumably within a short distance).</skos:example>
    </owl:Class>
    


    <!-- http://purl.org/poso/DeadReckoning -->


    <owl:Class rdf:about="http://purl.org/poso/DeadReckoning">
        <rdfs:subClassOf rdf:resource="http://purl.org/poso/PositioningTechnique"/>
        <rdfs:comment xml:lang="en">Dead reckoning is the Procedure of calculating the current position of a moving FeatureOfInterest by using its previous position and Sensor Observation&apos;s indicating its heading and velocity.</rdfs:comment>
        <rdfs:label xml:lang="en">Dead reckoning</rdfs:label>
        <skos:altLabel xml:lang="en">Deduced reckoning</skos:altLabel>
    </owl:Class>
    


    <!-- http://purl.org/poso/EulerOrientation -->


    <owl:Class rdf:about="http://purl.org/poso/EulerOrientation">
        <rdfs:subClassOf rdf:resource="http://purl.org/poso/Orientation"/>
        <rdfs:subClassOf>
            <owl:Restriction>
                <owl:onProperty rdf:resource="http://purl.org/poso/pitch"/>
                <owl:maxCardinality rdf:datatype="http://www.w3.org/2001/XMLSchema#nonNegativeInteger">1</owl:maxCardinality>
            </owl:Restriction>
        </rdfs:subClassOf>
        <rdfs:subClassOf>
            <owl:Restriction>
                <owl:onProperty rdf:resource="http://purl.org/poso/roll"/>
                <owl:maxCardinality rdf:datatype="http://www.w3.org/2001/XMLSchema#nonNegativeInteger">1</owl:maxCardinality>
            </owl:Restriction>
        </rdfs:subClassOf>
        <rdfs:subClassOf>
            <owl:Restriction>
                <owl:onProperty rdf:resource="http://purl.org/poso/yaw"/>
                <owl:maxCardinality rdf:datatype="http://www.w3.org/2001/XMLSchema#nonNegativeInteger">1</owl:maxCardinality>
            </owl:Restriction>
        </rdfs:subClassOf>
        <rdfs:label xml:lang="en">Euler orientation</rdfs:label>
    </owl:Class>
    


    <!-- http://purl.org/poso/Fingerprint -->


    <owl:Class rdf:about="http://purl.org/poso/Fingerprint">
        <owl:equivalentClass>
            <owl:Restriction>
                <owl:onProperty rdf:resource="http://purl.org/poso/hasPosition"/>
                <owl:qualifiedCardinality rdf:datatype="http://www.w3.org/2001/XMLSchema#nonNegativeInteger">1</owl:qualifiedCardinality>
                <owl:onClass rdf:resource="http://purl.org/poso/AbsolutePosition"/>
            </owl:Restriction>
        </owl:equivalentClass>
        <rdfs:subClassOf rdf:resource="http://www.w3.org/ns/sosa/FeatureOfInterest"/>
        <rdfs:subClassOf rdf:resource="http://www.w3.org/ns/sosa/Result"/>
        <rdfs:comment xml:lang="en">A fingerprint is a scene analysis at a particular absolute position.</rdfs:comment>
        <rdfs:label xml:lang="en">Fingerprint</rdfs:label>
    </owl:Class>
    


    <!-- http://purl.org/poso/Fingerprinting -->


    <owl:Class rdf:about="http://purl.org/poso/Fingerprinting">
        <rdfs:subClassOf rdf:resource="http://purl.org/poso/PositioningTechnique"/>
        <rdfs:comment xml:lang="en">Fingerprinting is a positioning Procedure where sensor data is collected at a specific position and orientation. During the offline-stage of a positioning system, the significant data features are extracted and stored for that position. In the online-stage, the closest match(es) of the features are determined to predict the position.</rdfs:comment>
        <rdfs:label xml:lang="en">Fingerprinting</rdfs:label>
    </owl:Class>
    


    <!-- http://purl.org/poso/HighLevelFusion -->


    <owl:Class rdf:about="http://purl.org/poso/HighLevelFusion">
        <rdfs:subClassOf rdf:resource="http://purl.org/poso/SensorFusion"/>
        <rdfs:comment xml:lang="en">High level sensor fusion is about fusing both objects and their trajectories. We&apos;re not only relying on detections, but also on predictions and tracking.</rdfs:comment>
        <rdfs:isDefinedBy rdf:datatype="http://www.w3.org/2001/XMLSchema#anyURI">https://www.thinkautonomous.ai/blog/?p=9-types-of-sensor-fusion-algorithms</rdfs:isDefinedBy>
        <rdfs:label xml:lang="en">High level sensor fusion</rdfs:label>
        <skos:altLabel xml:lang="en">Decision level sensor fusion</skos:altLabel>
    </owl:Class>
    


    <!-- http://purl.org/poso/IndoorDeployment -->


    <owl:Class rdf:about="http://purl.org/poso/IndoorDeployment">
        <rdfs:subClassOf rdf:resource="http://www.w3.org/ns/ssn/Deployment"/>
        <rdfs:comment xml:lang="en">Describes the spatial deployment of a System in an indoor environment.</rdfs:comment>
        <rdfs:label xml:lang="en">Indoor deployment</rdfs:label>
    </owl:Class>
    


    <!-- http://purl.org/poso/IndoorPositioningSystem -->


    <owl:Class rdf:about="http://purl.org/poso/IndoorPositioningSystem">
        <rdfs:subClassOf rdf:resource="http://purl.org/poso/PositioningSystem"/>
        <rdfs:comment xml:lang="en">A positioning system that is meant to perform indoor positioning of a feature of interest.</rdfs:comment>
        <rdfs:label xml:lang="en">Indoor positioning system</rdfs:label>
    </owl:Class>
    


    <!-- http://purl.org/poso/InertialPositioningSystem -->


    <owl:Class rdf:about="http://purl.org/poso/InertialPositioningSystem">
        <rdfs:subClassOf rdf:resource="http://purl.org/poso/PositioningSystem"/>
        <rdfs:comment xml:lang="en">An inertial positioning system is a positioning system employing accelerometers, gyroscopes, and computer as integral components to determine coordinates of points or objects relative to an initial known reference point</rdfs:comment>
        <rdfs:isDefinedBy rdf:datatype="http://www.w3.org/2001/XMLSchema#anyURI">https://isotc211.geolexica.org/concepts/240/</rdfs:isDefinedBy>
        <rdfs:label xml:lang="en">Inertial positioning system</rdfs:label>
    </owl:Class>
    


    <!-- http://purl.org/poso/IntegratedPositioningSystem -->


    <owl:Class rdf:about="http://purl.org/poso/IntegratedPositioningSystem">
        <rdfs:subClassOf rdf:resource="http://purl.org/poso/PositioningSystem"/>
        <rdfs:subClassOf>
            <owl:Restriction>
                <owl:onProperty rdf:resource="http://www.w3.org/ns/ssn/implements"/>
                <owl:minQualifiedCardinality rdf:datatype="http://www.w3.org/2001/XMLSchema#nonNegativeInteger">1</owl:minQualifiedCardinality>
                <owl:onClass rdf:resource="http://purl.org/poso/SensorFusion"/>
            </owl:Restriction>
        </rdfs:subClassOf>
        <rdfs:comment xml:lang="en">An integrated positioning system is a positioning system that incorporates multiple positioning technologies.</rdfs:comment>
        <rdfs:isDefinedBy rdf:datatype="http://www.w3.org/2001/XMLSchema#anyURI">https://isotc211.geolexica.org/concepts/250/</rdfs:isDefinedBy>
        <rdfs:label xml:lang="en">Integrated positioning system</rdfs:label>
        <skos:altLabel xml:lang="en">Hybrid positioning system</skos:altLabel>
    </owl:Class>
    


    <!-- http://purl.org/poso/Landmark -->


    <owl:Class rdf:about="http://purl.org/poso/Landmark">
        <rdfs:subClassOf rdf:resource="http://www.opengis.net/ont/geosparql#SpatialObject"/>
        <rdfs:subClassOf rdf:resource="http://www.w3.org/ns/sosa/FeatureOfInterest"/>
        <rdfs:subClassOf rdf:resource="http://www.w3.org/ns/sosa/Result"/>
        <rdfs:comment xml:lang="en">A landmark is a feature with a known position, that can be used to identify the position of an object that has a relative position with this feature.</rdfs:comment>
        <rdfs:label xml:lang="en">Landmark</rdfs:label>
    </owl:Class>
    


    <!-- http://purl.org/poso/Lateration -->


    <owl:Class rdf:about="http://purl.org/poso/Lateration">
        <rdfs:subClassOf rdf:resource="http://purl.org/poso/Triangulation"/>
        <rdfs:isDefinedBy rdf:datatype="http://www.w3.org/2001/XMLSchema#anyURI">https://www.sciencedirect.com/topics/engineering/lateration</rdfs:isDefinedBy>
        <rdfs:label xml:lang="en">Lateration</rdfs:label>
    </owl:Class>
    


    <!-- http://purl.org/poso/LinearAcceleration -->


    <owl:Class rdf:about="http://purl.org/poso/LinearAcceleration">
        <rdfs:subClassOf rdf:resource="http://purl.org/poso/Acceleration"/>
        <qudt:hasQuantityKind rdf:resource="http://qudt.org/vocab/quantitykind/LinearAcceleration"/>
        <rdfs:label xml:lang="en">Linear acceleration</rdfs:label>
    </owl:Class>
    


    <!-- http://purl.org/poso/LinearMovement -->


    <owl:Class rdf:about="http://purl.org/poso/LinearMovement">
        <rdfs:subClassOf rdf:resource="http://purl.org/poso/Movement"/>
        <rdfs:comment xml:lang="en">Linear movement along a certain axis.</rdfs:comment>
        <rdfs:label xml:lang="nl">Lineaire beweging</rdfs:label>
        <rdfs:label xml:lang="en">Linear movement</rdfs:label>
    </owl:Class>
    


    <!-- http://purl.org/poso/LinearVelocity -->


    <owl:Class rdf:about="http://purl.org/poso/LinearVelocity">
        <rdfs:subClassOf rdf:resource="http://purl.org/poso/Velocity"/>
        <qudt:hasQuantityKind rdf:resource="http://qudt.org/vocab/quantitykind/LinearVelocity"/>
        <rdfs:comment xml:lang="en">Linear velocity is the momentum along one ore more axis.</rdfs:comment>
        <rdfs:label xml:lang="nl">Lineaire snelheid</rdfs:label>
        <rdfs:label xml:lang="en">Linear velocity</rdfs:label>
    </owl:Class>
    


    <!-- http://purl.org/poso/LocationBasedService -->


    <owl:Class rdf:about="http://purl.org/poso/LocationBasedService">
        <rdfs:subClassOf rdf:resource="http://www.w3.org/ns/ssn/System"/>
        <rdfs:comment xml:lang="en">A location based service (LBS) is a service that provides the location of a person or object. It provides this information without the required knowledge of the underlying technologies and algorithms.</rdfs:comment>
        <rdfs:isDefinedBy rdf:datatype="http://www.w3.org/2001/XMLSchema#anyURI">https://isotc211.geolexica.org/concepts/278/</rdfs:isDefinedBy>
        <rdfs:label xml:lang="en">Location based service</rdfs:label>
    </owl:Class>
    


    <!-- http://purl.org/poso/LowLevelFusion -->


    <owl:Class rdf:about="http://purl.org/poso/LowLevelFusion">
        <rdfs:subClassOf rdf:resource="http://purl.org/poso/SensorFusion"/>
        <rdfs:comment xml:lang="en">Low Level Sensor Fusion is about fusing the raw data coming from multiple sensors. For example, we fuse point clouds coming from LiDARs and pixels coming from cameras.</rdfs:comment>
        <rdfs:isDefinedBy rdf:datatype="http://www.w3.org/2001/XMLSchema#anyURI">https://www.thinkautonomous.ai/blog/?p=9-types-of-sensor-fusion-algorithms</rdfs:isDefinedBy>
        <rdfs:label xml:lang="en">Low level sensor fusion</rdfs:label>
    </owl:Class>
    


    <!-- http://purl.org/poso/MagneticOdometry -->


    <owl:Class rdf:about="http://purl.org/poso/MagneticOdometry">
        <rdfs:subClassOf rdf:resource="http://purl.org/poso/Odometry"/>
        <rdfs:comment xml:lang="en">Magnetic field odometry is the procedure of detecting movement by analyizing how the magnetic field is changing from one Observation to another.</rdfs:comment>
        <rdfs:label xml:lang="en">Magnetic odometry</rdfs:label>
    </owl:Class>
    


    <!-- http://purl.org/poso/MapOutput -->


    <owl:Class rdf:about="http://purl.org/poso/MapOutput">
        <rdfs:subClassOf rdf:resource="http://www.w3.org/ns/ssn/Output"/>
        <rdfs:label xml:lang="en">Map output</rdfs:label>
    </owl:Class>
    


    <!-- http://purl.org/poso/MidLevelFusion -->


    <owl:Class rdf:about="http://purl.org/poso/MidLevelFusion">
        <rdfs:subClassOf rdf:resource="http://purl.org/poso/SensorFusion"/>
        <rdfs:comment xml:lang="en">Mid-Level sensor fusion is about fusing the objects detected independently on sensor data.</rdfs:comment>
        <rdfs:isDefinedBy rdf:datatype="http://www.w3.org/2001/XMLSchema#anyURI">https://www.thinkautonomous.ai/blog/?p=9-types-of-sensor-fusion-algorithms</rdfs:isDefinedBy>
        <rdfs:label xml:lang="en">Mid level sensor fusion</rdfs:label>
    </owl:Class>
    


    <!-- http://purl.org/poso/Movement -->


    <owl:Class rdf:about="http://purl.org/poso/Movement">
        <rdfs:subClassOf rdf:resource="http://www.w3.org/ns/ssn/Stimulus"/>
        <rdfs:comment xml:lang="en">Movement stimulus triggering an update of a position.</rdfs:comment>
        <rdfs:label xml:lang="nl">Beweging</rdfs:label>
        <rdfs:label xml:lang="en">Movement</rdfs:label>
    </owl:Class>
    


    <!-- http://purl.org/poso/Multilateration -->


    <owl:Class rdf:about="http://purl.org/poso/Multilateration">
        <rdfs:subClassOf rdf:resource="http://purl.org/poso/Lateration"/>
        <rdfs:comment xml:lang="en">Multilateration is the procedure of determining a position using relative distances to other known positions.</rdfs:comment>
        <rdfs:label xml:lang="en">Multilateration</rdfs:label>
        <skos:altLabel xml:lang="en">Hyperbolic positioning</skos:altLabel>
        <skos:altLabel xml:lang="en">Trilateration</skos:altLabel>
    </owl:Class>
    


    <!-- http://purl.org/poso/Odometry -->


    <owl:Class rdf:about="http://purl.org/poso/Odometry">
        <rdfs:subClassOf rdf:resource="http://purl.org/poso/PositioningTechnique"/>
        <rdfs:comment xml:lang="en">Odometry is the Procedure of calculating the current position of a moving FeatureOfInterest by using its previous position and Sensor Observation&apos;s indicating its heading and velocity.</rdfs:comment>
        <rdfs:label xml:lang="en">Odometry</rdfs:label>
    </owl:Class>
    


    <!-- http://purl.org/poso/OpticalPositioningSystem -->


    <owl:Class rdf:about="http://purl.org/poso/OpticalPositioningSystem">
        <rdfs:subClassOf rdf:resource="http://purl.org/poso/PositioningSystem"/>
        <rdfs:comment xml:lang="en">An optical positioning system is a positioning system that determines the position of an object by means of the properties of light.</rdfs:comment>
        <rdfs:isDefinedBy rdf:datatype="http://www.w3.org/2001/XMLSchema#anyURI">https://isotc211.geolexica.org/concepts/320/</rdfs:isDefinedBy>
        <rdfs:label xml:lang="en">Optical positioning system</rdfs:label>
    </owl:Class>
    


    <!-- http://purl.org/poso/Orientation -->


    <owl:Class rdf:about="http://purl.org/poso/Orientation">
        <rdfs:subClassOf rdf:resource="http://www.w3.org/ns/sosa/ObservableProperty"/>
        <rdfs:subClassOf rdf:resource="http://www.w3.org/ns/sosa/Result"/>
        <rdfs:comment xml:lang="nl">De orientatie van een object in 2D of 3D.</rdfs:comment>
        <rdfs:comment xml:lang="en">The orientation of a feature of interest in 2D or 3D space.</rdfs:comment>
        <rdfs:label xml:lang="nl">Orientatie</rdfs:label>
        <rdfs:label xml:lang="en">Orientation</rdfs:label>
    </owl:Class>
    


    <!-- http://purl.org/poso/OutdoorDeployment -->


    <owl:Class rdf:about="http://purl.org/poso/OutdoorDeployment">
        <rdfs:subClassOf rdf:resource="http://www.w3.org/ns/ssn/Deployment"/>
        <rdfs:comment xml:lang="en">Describes the deployment of a System in an outdoor environment.</rdfs:comment>
        <rdfs:label xml:lang="en">Outdoor deployment</rdfs:label>
    </owl:Class>
    


    <!-- http://purl.org/poso/PDR -->


    <owl:Class rdf:about="http://purl.org/poso/PDR">
        <rdfs:subClassOf rdf:resource="http://purl.org/poso/DeadReckoning"/>
        <rdfs:comment xml:lang="en">Pedestrian dead reckoning (PDR) is a positioning technique where the object is assumed to be a pedestrian that is walking or running. Using this knowledge, the dead reckoning involves the detection of steps and the step length to more accurately predict the movement.</rdfs:comment>
        <rdfs:label xml:lang="en">Pedestrian dead reckoning</rdfs:label>
    </owl:Class>
    


    <!-- http://purl.org/poso/PolygonalAccuracy -->


    <owl:Class rdf:about="http://purl.org/poso/PolygonalAccuracy">
        <rdfs:subClassOf rdf:resource="http://www.w3.org/ns/ssn/systems/Accuracy"/>
        <rdfs:label xml:lang="en">Polygonal accuracy</rdfs:label>
    </owl:Class>
    


    <!-- http://purl.org/poso/Position -->


    <owl:Class rdf:about="http://purl.org/poso/Position">
        <rdfs:subClassOf rdf:resource="http://www.w3.org/ns/sosa/ObservableProperty"/>
        <rdfs:subClassOf rdf:resource="http://www.w3.org/ns/sosa/Result"/>
        <rdfs:comment xml:lang="en">A position indicates where an entity is located.</rdfs:comment>
        <rdfs:label xml:lang="nl">Positie</rdfs:label>
        <rdfs:label xml:lang="en">Position</rdfs:label>
    </owl:Class>
    


    <!-- http://purl.org/poso/PositionOutput -->


    <owl:Class rdf:about="http://purl.org/poso/PositionOutput">
        <rdfs:subClassOf rdf:resource="http://www.w3.org/ns/ssn/Output"/>
        <rdfs:label xml:lang="en">Position output</rdfs:label>
    </owl:Class>
    


    <!-- http://purl.org/poso/PositioningPlatform -->


    <owl:Class rdf:about="http://purl.org/poso/PositioningPlatform">
        <rdfs:subClassOf rdf:resource="http://www.w3.org/ns/sosa/Platform"/>
        <rdfs:comment xml:lang="en">A positioning platform is a framework, architecture or platform used to develop and host a positioning system.</rdfs:comment>
        <rdfs:label xml:lang="en">Positioning platform</rdfs:label>
    </owl:Class>
    


    <!-- http://purl.org/poso/PositioningSystem -->


    <owl:Class rdf:about="http://purl.org/poso/PositioningSystem">
        <rdfs:subClassOf rdf:resource="http://www.w3.org/ns/ssn/System"/>
        <rdfs:subClassOf>
            <owl:Restriction>
                <owl:onProperty rdf:resource="http://www.w3.org/ns/ssn/hasDeployment"/>
                <owl:minQualifiedCardinality rdf:datatype="http://www.w3.org/2001/XMLSchema#nonNegativeInteger">1</owl:minQualifiedCardinality>
                <owl:onClass rdf:resource="http://www.w3.org/ns/ssn/Deployment"/>
            </owl:Restriction>
        </rdfs:subClassOf>
        <rdfs:comment xml:lang="en">A positioning system is a system of instrumental and computational components for determining position.</rdfs:comment>
        <rdfs:isDefinedBy rdf:datatype="http://www.w3.org/2001/XMLSchema#anyURI">https://isotc211.geolexica.org/concepts/349/</rdfs:isDefinedBy>
        <rdfs:label xml:lang="en">Positioning system</rdfs:label>
    </owl:Class>
    


    <!-- http://purl.org/poso/PositioningTechnique -->


    <owl:Class rdf:about="http://purl.org/poso/PositioningTechnique">
        <rdfs:subClassOf rdf:resource="http://www.w3.org/ns/sosa/Procedure"/>
        <rdfs:comment xml:lang="en">A positioning technique is a procedure to sample sensor data to an output position.</rdfs:comment>
        <rdfs:label xml:lang="en">Positioning technique</rdfs:label>
    </owl:Class>
    


    <!-- http://purl.org/poso/Proximity -->


    <owl:Class rdf:about="http://purl.org/poso/Proximity">
        <rdfs:subClassOf rdf:resource="http://www.w3.org/ns/ssn/Stimulus"/>
        <rdfs:comment xml:lang="en">Stimulus whenever two Feature of Interests are within close proximity.</rdfs:comment>
        <rdfs:label>Proximity</rdfs:label>
        <skos:example xml:lang="en">A Feature Of Interest can be within close proximity of another Feature Of Interest without movement whenever the other Feature moved wihin the proximity of the first Feature.</skos:example>
    </owl:Class>
    


    <!-- http://purl.org/poso/QuaternionOrientation -->


    <owl:Class rdf:about="http://purl.org/poso/QuaternionOrientation">
        <rdfs:subClassOf rdf:resource="http://purl.org/poso/Orientation"/>
        <rdfs:subClassOf>
            <owl:Restriction>
                <owl:onProperty rdf:resource="http://purl.org/poso/scalar"/>
                <owl:maxCardinality rdf:datatype="http://www.w3.org/2001/XMLSchema#nonNegativeInteger">1</owl:maxCardinality>
            </owl:Restriction>
        </rdfs:subClassOf>
        <rdfs:subClassOf>
            <owl:Restriction>
                <owl:onProperty rdf:resource="http://purl.org/poso/xAxisValue"/>
                <owl:maxCardinality rdf:datatype="http://www.w3.org/2001/XMLSchema#nonNegativeInteger">1</owl:maxCardinality>
            </owl:Restriction>
        </rdfs:subClassOf>
        <rdfs:subClassOf>
            <owl:Restriction>
                <owl:onProperty rdf:resource="http://purl.org/poso/yAxisValue"/>
                <owl:maxCardinality rdf:datatype="http://www.w3.org/2001/XMLSchema#nonNegativeInteger">1</owl:maxCardinality>
            </owl:Restriction>
        </rdfs:subClassOf>
        <rdfs:subClassOf>
            <owl:Restriction>
                <owl:onProperty rdf:resource="http://purl.org/poso/zAxisValue"/>
                <owl:maxCardinality rdf:datatype="http://www.w3.org/2001/XMLSchema#nonNegativeInteger">1</owl:maxCardinality>
            </owl:Restriction>
        </rdfs:subClassOf>
        <rdfs:label xml:lang="en">Quaternion orientation</rdfs:label>
    </owl:Class>
    


    <!-- http://purl.org/poso/RFLandmark -->


    <owl:Class rdf:about="http://purl.org/poso/RFLandmark">
        <rdfs:subClassOf rdf:resource="http://purl.org/poso/Landmark"/>
        <rdfs:comment xml:lang="en">A radio frequency landmark is a transmitting landmark that can be observed by its transmitting signals.</rdfs:comment>
        <rdfs:label xml:lang="en">RF landmark</rdfs:label>
        <skos:example xml:lang="en">An RF landmark example is a Bluetooth beacon that sends out a signal. Receivers of this signal can use the known position of this landmark to determine their relative position.</skos:example>
    </owl:Class>
    


    <!-- http://purl.org/poso/RadioPropagation -->


    <owl:Class rdf:about="http://purl.org/poso/RadioPropagation">
        <rdfs:subClassOf rdf:resource="http://www.w3.org/ns/sosa/Procedure"/>
        <rdfs:comment xml:lang="en">The radio propagation formulas cover the computation of the radio waves through a medium (e.g. air).</rdfs:comment>
        <rdfs:isDefinedBy rdf:datatype="http://www.w3.org/2001/XMLSchema#anyURI">https://en.wikipedia.org/wiki/Radio_propagation</rdfs:isDefinedBy>
        <rdfs:label xml:lang="en">Radio propagation</rdfs:label>
    </owl:Class>
    


    <!-- http://purl.org/poso/RelativeAngle -->


    <owl:Class rdf:about="http://purl.org/poso/RelativeAngle">
        <rdfs:subClassOf rdf:resource="http://purl.org/poso/RelativePosition"/>
        <rdfs:comment xml:lang="en">A relative angle is a quantitative angle relative to another feature of interest.</rdfs:comment>
        <rdfs:label xml:lang="nl">Relatieve hoek</rdfs:label>
        <rdfs:label xml:lang="en">Relative angle</rdfs:label>
        <skos:example xml:lang="en">An example of relative angle is the Angle of Arrival.</skos:example>
    </owl:Class>
    


    <!-- http://purl.org/poso/RelativeDistance -->


    <owl:Class rdf:about="http://purl.org/poso/RelativeDistance">
        <rdfs:subClassOf rdf:resource="http://purl.org/poso/RelativePosition"/>
        <rdfs:comment xml:lang="en">A relative distance is a quantitative distance relative to another feature of interest.</rdfs:comment>
        <rdfs:label xml:lang="nl">Relatieve afstand</rdfs:label>
        <rdfs:label xml:lang="en">Relative distance</rdfs:label>
    </owl:Class>
    


    <!-- http://purl.org/poso/RelativePosition -->


    <owl:Class rdf:about="http://purl.org/poso/RelativePosition">
        <rdfs:subClassOf rdf:resource="http://purl.org/poso/Position"/>
        <rdfs:subClassOf>
            <owl:Restriction>
                <owl:onProperty rdf:resource="http://purl.org/poso/isRelativeTo"/>
                <owl:maxQualifiedCardinality rdf:datatype="http://www.w3.org/2001/XMLSchema#nonNegativeInteger">1</owl:maxQualifiedCardinality>
                <owl:onClass rdf:resource="http://www.w3.org/ns/sosa/FeatureOfInterest"/>
            </owl:Restriction>
        </rdfs:subClassOf>
        <rdfs:comment xml:lang="en">A relative position is a position of a feature of interest with respect to the positions of other objects that this position is relative to.</rdfs:comment>
        <rdfs:comment xml:lang="nl">Een relatieve positie is een positie van een punt, met respect tot de posities van andere objecten die relatief zijn.</rdfs:comment>
        <rdfs:isDefinedBy rdf:datatype="http://www.w3.org/2001/XMLSchema#anyURI">https://isotc211.geolexica.org/concepts/377/</rdfs:isDefinedBy>
        <rdfs:label xml:lang="nl">Relatieve positie</rdfs:label>
        <rdfs:label xml:lang="en">Relative position</rdfs:label>
    </owl:Class>
    


    <!-- http://purl.org/poso/RelativeSignalStrength -->


    <owl:Class rdf:about="http://purl.org/poso/RelativeSignalStrength">
        <rdfs:subClassOf rdf:resource="http://purl.org/poso/RelativePosition"/>
        <rdfs:comment xml:lang="en">A relative signal strength is a received signal strength transmitted by another (RF) feature of interest.</rdfs:comment>
        <rdfs:label xml:lang="nl">Relatieve signaalsterkte</rdfs:label>
        <rdfs:label xml:lang="en">Relative signal strength</rdfs:label>
    </owl:Class>
    


    <!-- http://purl.org/poso/RelativeVelocity -->


    <owl:Class rdf:about="http://purl.org/poso/RelativeVelocity">
        <rdfs:subClassOf rdf:resource="http://purl.org/poso/RelativePosition"/>
        <rdfs:comment xml:lang="en">A relative velocity is a quantitative velocity relative to another feature of interest.</rdfs:comment>
        <rdfs:label xml:lang="nl">Relatieve snelheid</rdfs:label>
        <rdfs:label xml:lang="en">Relative velocity</rdfs:label>
    </owl:Class>
    


    <!-- http://purl.org/poso/SLAM -->


    <owl:Class rdf:about="http://purl.org/poso/SLAM">
        <rdfs:subClassOf rdf:resource="http://purl.org/poso/PositioningTechnique"/>
        <rdfs:comment xml:lang="en">Simultaneous localization and mapping (SLAM) is the computational problem of constructing or updating a map of an unknown environment while simultaneously keeping track of an agent&apos;s location within it.</rdfs:comment>
        <rdfs:isDefinedBy rdf:datatype="http://www.w3.org/2001/XMLSchema#anyURI">https://dbpedia.org/page/Simultaneous_localization_and_mapping</rdfs:isDefinedBy>
        <rdfs:label xml:lang="en">Simultaneous localisation and mapping</rdfs:label>
    </owl:Class>
    


    <!-- http://purl.org/poso/SRS -->


    <owl:Class rdf:about="http://purl.org/poso/SRS">
        <rdfs:subClassOf rdf:resource="http://www.w3.org/ns/ssn/systems/SystemProperty"/>
        <rdfs:comment xml:lang="en">An identifiable and observable spatial reference system that represents the System&apos;s ability to operate its primary purpose in a specified reference system.</rdfs:comment>
        <rdfs:label xml:lang="en">Spatial Reference System</rdfs:label>
    </owl:Class>
    


    <!-- http://purl.org/poso/SatellitePositioningSystem -->


    <owl:Class rdf:about="http://purl.org/poso/SatellitePositioningSystem">
        <rdfs:subClassOf rdf:resource="http://purl.org/poso/PositioningSystem"/>
        <rdfs:comment xml:lang="en">In this context, satellite positioning implies the use of radio signals transmitted from &quot;active&quot; artificial objects orbiting the Earth and received by &quot;passive&quot; instruments on or near the Earth&apos;s surface to determine position, velocity, and/or attitude of an object.</rdfs:comment>
        <rdfs:isDefinedBy rdf:datatype="http://www.w3.org/2001/XMLSchema#anyURI">https://isotc211.geolexica.org/concepts/392/</rdfs:isDefinedBy>
        <rdfs:label xml:lang="en">Satellite positioning system</rdfs:label>
    </owl:Class>
    


    <!-- http://purl.org/poso/SensorFusion -->


    <owl:Class rdf:about="http://purl.org/poso/SensorFusion">
        <rdfs:subClassOf rdf:resource="http://www.w3.org/ns/sosa/Procedure"/>
        <rdfs:comment xml:lang="en">Sensor fusion is a procedure where multiple sensor data is combined to obtain a more reliable or accurate result.</rdfs:comment>
        <rdfs:isDefinedBy rdf:datatype="http://www.w3.org/2001/XMLSchema#anyURI">https://en.wikipedia.org/wiki/Sensor_fusion</rdfs:isDefinedBy>
        <rdfs:label xml:lang="en">Sensor fusion</rdfs:label>
    </owl:Class>
    


    <!-- http://purl.org/poso/TrackedFeature -->


    <owl:Class rdf:about="http://purl.org/poso/TrackedFeature">
        <rdfs:subClassOf rdf:resource="http://www.opengis.net/ont/geosparql#SpatialObject"/>
        <rdfs:subClassOf rdf:resource="http://www.w3.org/ns/sosa/FeatureOfInterest"/>
        <rdfs:subClassOf>
            <owl:Restriction>
                <owl:onProperty rdf:resource="http://purl.org/poso/hasPosition"/>
                <owl:minQualifiedCardinality rdf:datatype="http://www.w3.org/2001/XMLSchema#nonNegativeInteger">1</owl:minQualifiedCardinality>
                <owl:onClass rdf:resource="http://purl.org/poso/Position"/>
            </owl:Restriction>
        </rdfs:subClassOf>
        <rdfs:comment xml:lang="en">A feature of interest that is being tracked by a positioning system. This is the feature for which a position is observed.</rdfs:comment>
        <rdfs:label xml:lang="en">Tracked feature</rdfs:label>
        <skos:example xml:lang="en">The phone of a person that is being tracked in an indoor positioning system is the tracked feature.</skos:example>
    </owl:Class>
    


    <!-- http://purl.org/poso/Triangulation -->


    <owl:Class rdf:about="http://purl.org/poso/Triangulation">
        <rdfs:subClassOf rdf:resource="http://purl.org/poso/PositioningTechnique"/>
        <rdfs:comment xml:lang="en">Triangulation is the procedure of determining a position using relative angles to a feature of interest with a known position.</rdfs:comment>
        <rdfs:label xml:lang="en">Triangulation</rdfs:label>
    </owl:Class>
    


    <!-- http://purl.org/poso/VSLAM -->


    <owl:Class rdf:about="http://purl.org/poso/VSLAM">
        <rdfs:subClassOf rdf:resource="http://purl.org/poso/SLAM"/>
        <rdfs:comment xml:lang="en">Visual simultaneous localisation and mapping (VSLAM) is a positioning techniques that uses visual imagery to map an environment. Positioning works by detecting features of interest in image frames and comparing how these features move from one frame to another.</rdfs:comment>
        <rdfs:label xml:lang="en">Visual simultaneous localisation and mapping</rdfs:label>
    </owl:Class>
    


    <!-- http://purl.org/poso/Velocity -->


    <owl:Class rdf:about="http://purl.org/poso/Velocity">
        <rdfs:subClassOf rdf:resource="http://www.w3.org/ns/sosa/ObservableProperty"/>
        <rdfs:subClassOf rdf:resource="http://www.w3.org/ns/sosa/Result"/>
        <qudt:hasQuantityKind rdf:resource="http://qudt.org/vocab/quantitykind/Velocity"/>
        <rdfs:comment xml:lang="en">Linear or angular velocity of a feature.</rdfs:comment>
        <rdfs:label xml:lang="en">Velocity</rdfs:label>
    </owl:Class>
    


    <!-- http://purl.org/poso/VisualInput -->


    <owl:Class rdf:about="http://purl.org/poso/VisualInput">
        <rdfs:subClassOf rdf:resource="http://www.w3.org/ns/ssn/Input"/>
        <rdfs:label xml:lang="en">Visual input</rdfs:label>
    </owl:Class>
    


    <!-- http://purl.org/poso/VisualLandmark -->


    <owl:Class rdf:about="http://purl.org/poso/VisualLandmark">
        <rdfs:subClassOf rdf:resource="http://purl.org/poso/Landmark"/>
        <rdfs:comment xml:lang="en">A visual landmark is a feature of interest that visually present in the space.</rdfs:comment>
        <rdfs:label xml:lang="en">Visual landmark</rdfs:label>
    </owl:Class>
    


    <!-- http://purl.org/poso/VisualOdometry -->


    <owl:Class rdf:about="http://purl.org/poso/VisualOdometry">
        <rdfs:subClassOf rdf:resource="http://purl.org/poso/Odometry"/>
        <rdfs:comment xml:lang="en">Visual odometry is the procedure of detecting movement by analyzing how visual features are moving from one Observation image frame to another.</rdfs:comment>
        <rdfs:label xml:lang="en">Visual odometry</rdfs:label>
    </owl:Class>
    


    <!-- http://www.opengis.net/ont/geosparql#Geometry -->


    <owl:Class rdf:about="http://www.opengis.net/ont/geosparql#Geometry"/>
    


    <!-- http://www.opengis.net/ont/geosparql#SpatialObject -->


    <owl:Class rdf:about="http://www.opengis.net/ont/geosparql#SpatialObject"/>
    


    <!-- http://www.w3.org/2000/01/rdf-schema#Class -->


    <owl:Class rdf:about="http://www.w3.org/2000/01/rdf-schema#Class"/>
    


    <!-- http://www.w3.org/ns/sosa/FeatureOfInterest -->


    <owl:Class rdf:about="http://www.w3.org/ns/sosa/FeatureOfInterest"/>
    


    <!-- http://www.w3.org/ns/ssn/System -->


    <owl:Class rdf:about="http://www.w3.org/ns/ssn/System"/>
</rdf:RDF>



<!-- Generated by the OWL API (version 5.1.18) https://github.com/owlcs/owlapi/ -->


