@prefix : <http://purl.org/poso/> .
@prefix owl: <http://www.w3.org/2002/07/owl#> .
@prefix rdf: <http://www.w3.org/1999/02/22-rdf-syntax-ns#> .
@prefix xml: <http://www.w3.org/XML/1998/namespace> .
@prefix xsd: <http://www.w3.org/2001/XMLSchema#> .
@prefix rdfs: <http://www.w3.org/2000/01/rdf-schema#> .
@prefix skos: <http://www.w3.org/2004/02/skos/core#> .
@base <http://purl.org/poso/> .

<http://purl.org/poso/> rdf:type owl:Ontology ;
                         owl:versionIRI <http://purl.org/poso/1.1/> ;
                         owl:imports <http://www.w3.org/ns/ssn/> ,
                                     <http://www.w3.org/ns/ssn/systems/> ;
                         <http://purl.org/dc/terms/abstract> "The positioning system ontology is a vocabulary for describing positioning systems and the techniques these systems use to determine a position. With POSO we aim to provide semantic meaning on how a positioning system is deployed and how results are calculated."@en ;
                         <http://purl.org/dc/terms/bibliographicCitation> "Maxim Van de Wynckel and Beat Signer, POSO: A Generic Positioning System Ontology"^^xsd:string ;
                         <http://purl.org/dc/terms/contributor> "Beat Signer"@en ;
                         <http://purl.org/dc/terms/creator> "Maxim Van de Wynckel"@en ;
                         <http://purl.org/dc/terms/description> "This ontology provides the terminologies used for positioning systems." ;
                         <http://purl.org/dc/terms/license> <http://purl.org/NET/rdflicense/MIT1.0> ;
                         <http://purl.org/dc/terms/modified> "2024-12-16T00:00:00"^^xsd:dateTime ;
                         <http://purl.org/dc/terms/title> "Positioning System Ontology"@en ;
                         <http://purl.org/vocab/vann/preferredNamespacePrefix> "poso" ;
                         <http://purl.org/vocab/vann/preferredNamespaceUri> "http://purl.org/poso/"^^xsd:anyURI ;
                         <http://schema.org/image> "https://raw.githubusercontent.com/OpenHPS/POSO/main/1.1/docs/images/systems_and_procedures.svg" .

#################################################################
#    Annotation properties
#################################################################

###  http://purl.org/dc/terms/abstract
<http://purl.org/dc/terms/abstract> rdf:type owl:AnnotationProperty .


###  http://purl.org/dc/terms/bibliographicCitation
<http://purl.org/dc/terms/bibliographicCitation> rdf:type owl:AnnotationProperty .


###  http://purl.org/dc/terms/contributor
<http://purl.org/dc/terms/contributor> rdf:type owl:AnnotationProperty .


###  http://purl.org/dc/terms/creator
<http://purl.org/dc/terms/creator> rdf:type owl:AnnotationProperty .


###  http://purl.org/dc/terms/description
<http://purl.org/dc/terms/description> rdf:type owl:AnnotationProperty .


###  http://purl.org/dc/terms/license
<http://purl.org/dc/terms/license> rdf:type owl:AnnotationProperty .


###  http://purl.org/dc/terms/modified
<http://purl.org/dc/terms/modified> rdf:type owl:AnnotationProperty .


###  http://purl.org/dc/terms/source
<http://purl.org/dc/terms/source> rdf:type owl:AnnotationProperty .


###  http://purl.org/dc/terms/title
<http://purl.org/dc/terms/title> rdf:type owl:AnnotationProperty .


###  http://purl.org/vocab/vann/preferredNamespacePrefix
<http://purl.org/vocab/vann/preferredNamespacePrefix> rdf:type owl:AnnotationProperty .


###  http://purl.org/vocab/vann/preferredNamespaceUri
<http://purl.org/vocab/vann/preferredNamespaceUri> rdf:type owl:AnnotationProperty .


###  http://qudt.org/schema/qudt/example
<http://qudt.org/schema/qudt/example> rdf:type owl:AnnotationProperty .


###  http://qudt.org/schema/qudt/hasQuantityKind
<http://qudt.org/schema/qudt/hasQuantityKind> rdf:type owl:AnnotationProperty .


###  http://schema.org/image
<http://schema.org/image> rdf:type owl:AnnotationProperty .


###  http://www.w3.org/2004/02/skos/core#altLabel
skos:altLabel rdf:type owl:AnnotationProperty .


#################################################################
#    Object Properties
#################################################################

###  http://purl.org/poso/angle
:angle rdf:type owl:ObjectProperty ,
                owl:FunctionalProperty ;
       rdfs:domain <http://www.w3.org/ns/sosa/Result> ;
       rdfs:range rdfs:Class ;
       rdfs:comment "Quantitative angle result value for axis-angle representation."@en ;
       rdfs:label "angle"@en ,
                  "hoek"@nl .


###  http://purl.org/poso/hasAcceleration
:hasAcceleration rdf:type owl:ObjectProperty ;
                 rdfs:subPropertyOf <http://www.w3.org/ns/ssn/hasProperty> ;
                 owl:inverseOf :isAccelerationOf ;
                 rdfs:domain <http://www.w3.org/ns/sosa/FeatureOfInterest> ;
                 rdfs:range :Acceleration ;
                 rdfs:comment "Property that links a feature of interest to a unique acceleration property related to this feature."@en ;
                 rdfs:label "has acceleration"@en ,
                            "heeft versnelling"@nl .


###  http://purl.org/poso/hasAccuracy
:hasAccuracy rdf:type owl:ObjectProperty ;
             rdfs:subPropertyOf <http://www.w3.org/ns/ssn/hasProperty> ;
             rdf:type owl:FunctionalProperty ;
             rdfs:comment "The accuracy of an entity."@en ;
             rdfs:label "has accuracy"@en ,
                        "heeft accuraatheid"@nl .


###  http://purl.org/poso/hasCRS
:hasCRS rdf:type owl:ObjectProperty ;
        rdfs:subPropertyOf :hasSRS ;
        rdfs:label "has coordinate reference system"@en ,
                   "heeft een co√∂rdinaten referentiesysteem"@nl .


###  http://purl.org/poso/hasOrientation
:hasOrientation rdf:type owl:ObjectProperty ;
                rdfs:subPropertyOf <http://www.w3.org/ns/ssn/hasProperty> ;
                owl:inverseOf :isOrientationOf ;
                rdfs:domain <http://www.w3.org/ns/sosa/FeatureOfInterest> ;
                rdfs:range :Orientation ;
                rdfs:comment "Duid de orientatie aan van een object aan."@nl ,
                             "Indicates the orientation of a feature of interest."@en ;
                rdfs:label "has orientation"@en ,
                           "heeft orientatie"@nl .


###  http://purl.org/poso/hasPosition
:hasPosition rdf:type owl:ObjectProperty ;
             rdfs:subPropertyOf <http://www.w3.org/ns/ssn/hasProperty> ;
             owl:inverseOf :isPositionOf ;
             rdfs:domain <http://www.w3.org/ns/sosa/FeatureOfInterest> ;
             rdfs:range :Position ;
             rdfs:comment "Duid de absolute of relatieve positie van een object aan."@nl ,
                          "Indicates the absolute or relative position of a feature of interest."@en ;
             rdfs:label "has position"@en ,
                        "heeft positie"@nl .


###  http://purl.org/poso/hasRSS
:hasRSS rdf:type owl:ObjectProperty ;
        rdfs:subPropertyOf :hasRelativePosition ;
        rdfs:range :RelativeSignalStrength ;
        rdfs:label "has relative signal strength"@en .


###  http://purl.org/poso/hasRelativeDistance
:hasRelativeDistance rdf:type owl:ObjectProperty ;
                     rdfs:subPropertyOf :hasRelativePosition ;
                     rdfs:range :RelativeDistance ;
                     rdfs:label "has relative distance"@en .


###  http://purl.org/poso/hasRelativePosition
:hasRelativePosition rdf:type owl:ObjectProperty ;
                     rdfs:subPropertyOf :hasPosition ;
                     owl:inverseOf :isRelativeTo ;
                     rdfs:range :RelativePosition ;
                     rdfs:label "has relative position"@en ,
                                "heeft relatieve positie"@nl .


###  http://purl.org/poso/hasSRS
:hasSRS rdf:type owl:ObjectProperty ;
        rdfs:domain owl:Thing ;
        <http://qudt.org/schema/qudt/example> <http://www.opengis.net/def/crs/OGC/1.3/CRS84> ;
        rdfs:comment "Identifies an entity that has a spatial reference system in order to interpret the result."@en ;
        rdfs:label "has spatial reference system"@en ,
                   "heeft een ruimtelijk referentiepunt"@nl .


###  http://purl.org/poso/hasVelocity
:hasVelocity rdf:type owl:ObjectProperty ;
             rdfs:subPropertyOf <http://www.w3.org/ns/ssn/hasProperty> ;
             owl:inverseOf :isVelocityOf ;
             rdfs:domain <http://www.w3.org/ns/sosa/FeatureOfInterest> ;
             rdfs:range :Velocity ;
             rdfs:comment "Duid de snelheid van een object aan."@nl ,
                          "Indicates the velocity of a feature of interest."@en ;
             rdfs:label "has velocity"@en ,
                        "heeft snelheid"@nl .


###  http://purl.org/poso/inDeployment
:inDeployment rdf:type owl:ObjectProperty ;
              rdfs:domain :AbsolutePosition ;
              rdfs:range <http://www.w3.org/ns/ssn/Deployment> ;
              <http://purl.org/vocab/vann/preferredNamespaceUri> "Identifies an absolute position within a deployment"@en ;
              rdfs:label "in deployment"@en .


###  http://purl.org/poso/isAccelerationOf
:isAccelerationOf rdf:type owl:ObjectProperty ;
                  rdfs:subPropertyOf <http://www.w3.org/ns/ssn/isPropertyOf> ;
                  rdfs:label "is acceleration of"@en ,
                             "is versnelling van"@nl .


###  http://purl.org/poso/isOrientationOf
:isOrientationOf rdf:type owl:ObjectProperty ;
                 rdfs:subPropertyOf <http://www.w3.org/ns/ssn/isPropertyOf> ;
                 rdfs:label "is orientatie van"@nl ,
                            "is orientation of"@en .


###  http://purl.org/poso/isPositionOf
:isPositionOf rdf:type owl:ObjectProperty ;
              rdfs:subPropertyOf <http://www.w3.org/ns/ssn/isPropertyOf> ;
              rdfs:label "is positie van"@nl ,
                         "is position of"@en .


###  http://purl.org/poso/isRelativeTo
:isRelativeTo rdf:type owl:ObjectProperty ;
              rdfs:domain :AbsolutePosition ,
                          :Orientation ,
                          :RelativePosition ;
              rdfs:range <http://www.w3.org/ns/sosa/FeatureOfInterest> ;
              rdfs:comment "Indicates a position or orientation to be relative to another feature of interest."@en ;
              rdfs:label "is relatief met"@nl ,
                         "is relative to"@en ;
              skos:example "A person can have a relative distance to another feature of interest. When a feature is moving (i.e. when the geometry changes based on time) the distance remains relative to the feature and not the geometry at a specific point in time."@en .


###  http://purl.org/poso/isVelocityOf
:isVelocityOf rdf:type owl:ObjectProperty ;
              rdfs:subPropertyOf <http://www.w3.org/ns/ssn/isPropertyOf> ;
              rdfs:label "is de snelheid van"@nl ,
                         "is velocity of"@en .


###  http://purl.org/poso/madeByProcedure
:madeByProcedure rdf:type owl:ObjectProperty ;
                 rdfs:domain <http://www.w3.org/ns/ssn/Input> ;
                 rdfs:range <http://www.w3.org/ns/sosa/Procedure> ;
                 rdfs:comment "Input type outputted by another procedure"@en ;
                 rdfs:label "made by procecure"@en .


###  http://purl.org/poso/madeBySystem
:madeBySystem rdf:type owl:ObjectProperty ;
              rdfs:domain <http://www.w3.org/ns/sosa/Observation> ;
              rdfs:range <http://www.w3.org/ns/ssn/System> ;
              rdfs:comment "A relation to a re-usable system that computed the observation."@en ;
              rdfs:label "gemaakt door systeem"@nl ,
                         "made by system"@en .


###  http://purl.org/poso/nutation
:nutation rdf:type owl:ObjectProperty ;
          rdfs:domain :EulerOrientation ;
          rdfs:label "nutation"@en .


###  http://purl.org/poso/observesType
:observesType rdf:type owl:ObjectProperty ;
              rdfs:subPropertyOf <http://www.w3.org/ns/ssn/forProperty> ;
              rdfs:domain <http://www.w3.org/ns/ssn/System> ;
              rdfs:range rdfs:Class ;
              rdfs:comment "The relation between a system and an observable property class to identify that a system observes a specific type of property."@en ;
              rdfs:label "observeert type"@nl ,
                         "observes type"@en .


###  http://purl.org/poso/order
:order rdf:type owl:ObjectProperty ;
       rdfs:domain :EulerOrientation ;
       rdfs:range :EulerOrder ;
       rdfs:label "order"@en .


###  http://purl.org/poso/pitch
:pitch rdf:type owl:ObjectProperty ,
                owl:FunctionalProperty ;
       rdfs:domain :EulerOrientation ;
       rdfs:range owl:Thing ;
       rdfs:comment "Pitch is the rotation around the axis with respect to the object the yaw applies to."@en ;
       rdfs:label "pitch"@en .


###  http://purl.org/poso/precession
:precession rdf:type owl:ObjectProperty ;
            rdfs:domain :EulerOrientation ;
            rdfs:label "precession"@en .


###  http://purl.org/poso/roll
:roll rdf:type owl:ObjectProperty ,
               owl:FunctionalProperty ;
      rdfs:domain :EulerOrientation ;
      rdfs:range owl:Thing ;
      rdfs:comment "Roll is the rotation around the axis with respect to the object the roll applies to."@en ;
      rdfs:label "roll"@en .


###  http://purl.org/poso/scalar
:scalar rdf:type owl:ObjectProperty ,
                 owl:FunctionalProperty ;
        rdfs:domain <http://www.w3.org/ns/sosa/Result> ;
        rdfs:range owl:Thing ;
        rdfs:label "scalar"@en ;
        skos:altLabel "w" .


###  http://purl.org/poso/spin
:spin rdf:type owl:ObjectProperty ;
      rdfs:domain :EulerOrientation ;
      rdfs:label "spin"@en .


###  http://purl.org/poso/xAxisValue
:xAxisValue rdf:type owl:ObjectProperty ,
                     owl:FunctionalProperty ;
            rdfs:domain <http://www.w3.org/ns/sosa/Result> ;
            rdfs:range owl:Thing ;
            rdfs:comment "Quantitative result value along the X-axis of a spatial sensor or result."@en ;
            rdfs:label "x-axis value"@en .


###  http://purl.org/poso/yAxisValue
:yAxisValue rdf:type owl:ObjectProperty ,
                     owl:FunctionalProperty ;
            rdfs:domain <http://www.w3.org/ns/sosa/Result> ;
            rdfs:range rdfs:Class ;
            rdfs:comment "Quantitative result value along the Y-axis of a spatial sensor or result."@en ;
            rdfs:label "y-axis value"@en .


###  http://purl.org/poso/yaw
:yaw rdf:type owl:ObjectProperty ,
              owl:FunctionalProperty ;
     rdfs:domain :EulerOrientation ;
     rdfs:range owl:Thing ;
     rdfs:comment "Yaw is the rotation around the axis with respect to the object the yaw applies to."@en ;
     rdfs:label "yaw"@en .


###  http://purl.org/poso/zAxisValue
:zAxisValue rdf:type owl:ObjectProperty ,
                     owl:FunctionalProperty ;
            rdfs:domain <http://www.w3.org/ns/sosa/Result> ;
            rdfs:range owl:Thing ;
            rdfs:comment "Quantitative result value along the Z-axis of a spatial sensor."@en ;
            rdfs:label "z-axis value"@en .


#################################################################
#    Classes
#################################################################

###  http://purl.org/poso/AbsolutePosition
:AbsolutePosition rdf:type owl:Class ;
                  owl:equivalentClass <http://www.opengis.net/ont/geosparql#Geometry> ;
                  rdfs:subClassOf :Position ;
                  rdfs:comment "An absolute position describes the position of an entity based on a fixed point in space. Usually this space is the Earth and the position is expressed in latitude and longitude."@en ;
                  rdfs:label "Absolute position"@en .


###  http://purl.org/poso/Acceleration
:Acceleration rdf:type owl:Class ;
              rdfs:subClassOf <http://www.w3.org/ns/sosa/ObservableProperty> ,
                              <http://www.w3.org/ns/sosa/Result> ;
              <http://qudt.org/schema/qudt/hasQuantityKind> <http://qudt.org/vocab/quantitykind/Acceleration> ;
              rdfs:comment "Acceleration is the (instantaneous) rate of change of velocity."@en ;
              rdfs:label "Acceleration"@en ,
                         "Versnelling"@nl .


###  http://purl.org/poso/AngularAcceleration
:AngularAcceleration rdf:type owl:Class ;
                     rdfs:subClassOf :Acceleration ;
                     <http://qudt.org/schema/qudt/hasQuantityKind> <http://qudt.org/vocab/quantitykind/AngularAcceleration> ;
                     rdfs:label "Angular acceleration"@en ,
                                "Draaiversnelling"@nl .


###  http://purl.org/poso/AngularMotion
:AngularMotion rdf:type owl:Class ;
               rdfs:subClassOf :Motion ;
               rdfs:comment "Angular motion around a certain origin point."@en ;
               rdfs:label "Angular motion"@en ,
                          "Draaibeweging"@nl .


###  http://purl.org/poso/AngularVelocity
:AngularVelocity rdf:type owl:Class ;
                 rdfs:subClassOf :Velocity ;
                 <http://qudt.org/schema/qudt/hasQuantityKind> <http://qudt.org/vocab/quantitykind/AngularVelocity> ;
                 rdfs:comment "Angular velocity is the momentum around a point of origin."@en ;
                 rdfs:label "Angular velocity"@en ,
                            "Draaisnelheid"@nl .


###  http://purl.org/poso/Angulation
:Angulation rdf:type owl:Class ;
            rdfs:subClassOf :PositioningTechnique ;
            rdfs:comment "Angle-based positioning techniques are positioning techniques that use angles to determine a position."@en ;
            rdfs:label "Angulation"@en ;
            skos:altLabel "Angle-based positioning techniques"@en .


###  http://purl.org/poso/AuditoryLandmark
:AuditoryLandmark rdf:type owl:Class ;
                  rdfs:subClassOf :Landmark ;
                  rdfs:comment "A spatial landmark that can be observed by sound."@en ;
                  rdfs:label "Auditory landmark"@en .


###  http://purl.org/poso/AxisAngleOrientation
:AxisAngleOrientation rdf:type owl:Class ;
                      rdfs:subClassOf :Orientation ,
                                      [ rdf:type owl:Restriction ;
                                        owl:onProperty :angle ;
                                        owl:minCardinality "1"^^xsd:nonNegativeInteger
                                      ] ,
                                      [ rdf:type owl:Restriction ;
                                        owl:onProperty :angle ;
                                        owl:maxCardinality "1"^^xsd:nonNegativeInteger
                                      ] ,
                                      [ rdf:type owl:Restriction ;
                                        owl:onProperty :xAxisValue ;
                                        owl:maxCardinality "1"^^xsd:nonNegativeInteger
                                      ] ,
                                      [ rdf:type owl:Restriction ;
                                        owl:onProperty :yAxisValue ;
                                        owl:maxCardinality "1"^^xsd:nonNegativeInteger
                                      ] ,
                                      [ rdf:type owl:Restriction ;
                                        owl:onProperty :zAxisValue ;
                                        owl:maxCardinality "1"^^xsd:nonNegativeInteger
                                      ] ;
                      rdfs:comment "The axis-angle orientation is an orientation representation where the x, y and z values are rotated with a certain angle."@en ;
                      rdfs:label "Axis-angle orientation"@en .


###  http://purl.org/poso/Beamforming
:Beamforming rdf:type owl:Class ;
             rdfs:subClassOf :Angulation ;
             rdfs:comment "Beamforming is a signal processing technique that uses an array of antennas to form a directional beam of radio waves. By adjusting the direction of the beam and measuring the angle of arrival or departure of the signal, the position of a receiver can be estimated."@en ;
             rdfs:isDefinedBy "https://ieeexplore.ieee.org/document/9369486"^^xsd:anyURI ;
             rdfs:label "Beamforming"@en .


###  http://purl.org/poso/BluetoothBeacon
:BluetoothBeacon rdf:type owl:Class ;
                 rdfs:subClassOf :RFLandmark ;
                 rdfs:comment "A Bluetooth beacon is an RF landmark that advertises its transmission power and other optional information. Based on the signal strength receivers of this advertisement can determine the approximate distance."@en ;
                 rdfs:label "Bluetooth beacon"@en .


###  http://purl.org/poso/BluetoothReceiver
:BluetoothReceiver rdf:type owl:Class ;
                   rdfs:subClassOf :RFLandmark ;
                   rdfs:label "Bluetooth receiver"@en .


###  http://purl.org/poso/CalibrationMagnitudeProcedure
:CalibrationMagnitudeProcedure rdf:type owl:Class ;
                               rdfs:subClassOf :NormalizationProcedure ;
                               rdfs:label "Calibration magnitude procedure"@en .


###  http://purl.org/poso/CalibrationOffsetProcedure
:CalibrationOffsetProcedure rdf:type owl:Class ;
                            rdfs:subClassOf :NormalizationProcedure ;
                            rdfs:label "Calibration offset procedure"@en .


###  http://purl.org/poso/CalibrationProcedure
:CalibrationProcedure rdf:type owl:Class ;
                      rdfs:subClassOf <http://www.w3.org/ns/sosa/Procedure> ;
                      rdfs:comment "Calibration is the act of using sensor data obtained by a user to configure a system to output data with a reliable result."@en ;
                      rdfs:label "Calibration procedure"@en .


###  http://purl.org/poso/CellIdentification
:CellIdentification rdf:type owl:Class ;
                    rdfs:subClassOf :PositioningTechnique ;
                    rdfs:comment "Cell identification is a positioning procedure using the position of one landmark that is within the cell."@en ;
                    rdfs:label "Cell identification"@en ;
                    skos:altLabel "Cell Of Origin (COO)"@en ;
                    skos:example "An example of cell identification is using the position of a Bluetooth beacon whenever this beacon has a high signal strength."@en ,
                                 "An example of cell identification is using the position of a QR-code when this code is scanned (and the user is presumably within a short distance)."@en .


###  http://purl.org/poso/DeadReckoning
:DeadReckoning rdf:type owl:Class ;
               rdfs:subClassOf :PositioningTechnique ;
               rdfs:comment "Dead reckoning is the Procedure of calculating the current position of a moving FeatureOfInterest by using its previous position and Sensor Observation's indicating its heading and velocity."@en ;
               rdfs:label "Dead reckoning"@en ;
               skos:altLabel "Deduced reckoning"@en .


###  http://purl.org/poso/EulerOrder
:EulerOrder rdf:type owl:Class ;
            rdfs:comment "The order in which to apply Euler rotations."@en ;
            rdfs:label "Euler order"@en .


###  http://purl.org/poso/EulerOrientation
:EulerOrientation rdf:type owl:Class ;
                  rdfs:subClassOf :Orientation ,
                                  [ rdf:type owl:Restriction ;
                                    owl:onProperty :order ;
                                    owl:minQualifiedCardinality "1"^^xsd:nonNegativeInteger ;
                                    owl:onClass :EulerOrder
                                  ] ,
                                  [ rdf:type owl:Restriction ;
                                    owl:onProperty :nutation ;
                                    owl:maxCardinality "1"^^xsd:nonNegativeInteger
                                  ] ,
                                  [ rdf:type owl:Restriction ;
                                    owl:onProperty :pitch ;
                                    owl:maxCardinality "1"^^xsd:nonNegativeInteger
                                  ] ,
                                  [ rdf:type owl:Restriction ;
                                    owl:onProperty :precession ;
                                    owl:maxCardinality "1"^^xsd:nonNegativeInteger
                                  ] ,
                                  [ rdf:type owl:Restriction ;
                                    owl:onProperty :roll ;
                                    owl:maxCardinality "1"^^xsd:nonNegativeInteger
                                  ] ,
                                  [ rdf:type owl:Restriction ;
                                    owl:onProperty :spin ;
                                    owl:maxCardinality "1"^^xsd:nonNegativeInteger
                                  ] ,
                                  [ rdf:type owl:Restriction ;
                                    owl:onProperty :yaw ;
                                    owl:maxCardinality "1"^^xsd:nonNegativeInteger
                                  ] ;
                  rdfs:label "Euler orientation"@en .


###  http://purl.org/poso/Fingerprint
:Fingerprint rdf:type owl:Class ;
             owl:equivalentClass [ rdf:type owl:Restriction ;
                                   owl:onProperty :hasPosition ;
                                   owl:qualifiedCardinality "1"^^xsd:nonNegativeInteger ;
                                   owl:onClass :AbsolutePosition
                                 ] ;
             rdfs:subClassOf <http://www.w3.org/ns/sosa/FeatureOfInterest> ,
                             <http://www.w3.org/ns/sosa/Result> ;
             rdfs:comment "A fingerprint is a scene analysis at a particular absolute position."@en ;
             rdfs:label "Fingerprint"@en .


###  http://purl.org/poso/Fingerprinting
:Fingerprinting rdf:type owl:Class ;
                rdfs:subClassOf :PositioningTechnique ;
                rdfs:comment "Fingerprinting is a positioning Procedure where sensor data is collected at a specific position and orientation. During the offline-stage of a positioning system, the significant data features are extracted and stored for that position. In the online-stage, the closest match(es) of the features are determined to predict the position."@en ;
                rdfs:label "Fingerprinting"@en .


###  http://purl.org/poso/HighLevelFusion
:HighLevelFusion rdf:type owl:Class ;
                 rdfs:subClassOf :SensorFusion ;
                 rdfs:comment "High level sensor fusion is about fusing both objects and their trajectories. We're not only relying on detections, but also on predictions and tracking."@en ;
                 rdfs:isDefinedBy "https://www.thinkautonomous.ai/blog/?p=9-types-of-sensor-fusion-algorithms"^^xsd:anyURI ;
                 rdfs:label "High level sensor fusion"@en ;
                 skos:altLabel "Decision level sensor fusion"@en .


###  http://purl.org/poso/HybridDeployment
:HybridDeployment rdf:type owl:Class ;
                  rdfs:subClassOf <http://www.w3.org/ns/ssn/Deployment> ;
                  rdfs:comment "A hybrid deployment covers an indoor and outdoor deployment."@en ;
                  rdfs:label "Hybrid deployment"@en .


###  http://purl.org/poso/IndoorDeployment
:IndoorDeployment rdf:type owl:Class ;
                  rdfs:subClassOf <http://www.w3.org/ns/ssn/Deployment> ;
                  rdfs:comment "Describes the spatial deployment of a System in an indoor environment."@en ;
                  rdfs:label "Indoor deployment"@en .


###  http://purl.org/poso/IndoorPositioningSystem
:IndoorPositioningSystem rdf:type owl:Class ;
                         rdfs:subClassOf :PositioningSystem ;
                         rdfs:comment "A positioning system that is meant to perform indoor positioning of a feature of interest."@en ;
                         rdfs:label "Indoor positioning system"@en .


###  http://purl.org/poso/InertialPositioningSystem
:InertialPositioningSystem rdf:type owl:Class ;
                           rdfs:subClassOf :PositioningSystem ;
                           rdfs:comment "An inertial positioning system is a positioning system employing accelerometers, gyroscopes, and computer as integral components to determine coordinates of points or objects relative to an initial known reference point"@en ;
                           rdfs:isDefinedBy "https://isotc211.geolexica.org/concepts/240/"^^xsd:anyURI ;
                           rdfs:label "Inertial positioning system"@en .


###  http://purl.org/poso/IntegratedPositioningSystem
:IntegratedPositioningSystem rdf:type owl:Class ;
                             rdfs:subClassOf :PositioningSystem ,
                                             [ rdf:type owl:Restriction ;
                                               owl:onProperty <http://www.w3.org/ns/ssn/implements> ;
                                               owl:minQualifiedCardinality "1"^^xsd:nonNegativeInteger ;
                                               owl:onClass :SensorFusion
                                             ] ;
                             rdfs:comment "An integrated positioning system is a positioning system that incorporates multiple positioning technologies."@en ;
                             rdfs:isDefinedBy "https://isotc211.geolexica.org/concepts/250/"^^xsd:anyURI ;
                             rdfs:label "Integrated positioning system"@en ;
                             skos:altLabel "Hybrid positioning system"@en .


###  http://purl.org/poso/Landmark
:Landmark rdf:type owl:Class ;
          rdfs:subClassOf <http://www.opengis.net/ont/geosparql#SpatialObject> ,
                          <http://www.w3.org/ns/sosa/FeatureOfInterest> ,
                          <http://www.w3.org/ns/sosa/Result> ;
          rdfs:comment "A landmark is a feature with a known position, that can be used to identify the position of an object that has a relative position with this feature."@en ;
          rdfs:label "Landmark"@en .


###  http://purl.org/poso/Lateration
:Lateration rdf:type owl:Class ;
            rdfs:subClassOf :PositioningTechnique ;
            rdfs:isDefinedBy "https://www.sciencedirect.com/topics/engineering/lateration"^^xsd:anyURI ;
            rdfs:label "Lateration"@en ;
            skos:altLabel "Distance-based positioning"@en .


###  http://purl.org/poso/LinearAcceleration
:LinearAcceleration rdf:type owl:Class ;
                    rdfs:subClassOf :Acceleration ;
                    <http://qudt.org/schema/qudt/hasQuantityKind> <http://qudt.org/vocab/quantitykind/LinearAcceleration> ;
                    rdfs:label "Linear acceleration"@en .


###  http://purl.org/poso/LinearMotion
:LinearMotion rdf:type owl:Class ;
              rdfs:subClassOf :Motion ;
              rdfs:comment "Linear motion along a certain axis."@en ;
              rdfs:label "Lineaire beweging"@nl ,
                         "Linear motion"@en .


###  http://purl.org/poso/LinearVelocity
:LinearVelocity rdf:type owl:Class ;
                rdfs:subClassOf :Velocity ;
                <http://qudt.org/schema/qudt/hasQuantityKind> <http://qudt.org/vocab/quantitykind/LinearVelocity> ;
                rdfs:comment "Linear velocity is the momentum along one ore more axis."@en ;
                rdfs:label "Lineaire snelheid"@nl ,
                           "Linear velocity"@en .


###  http://purl.org/poso/LocationBasedService
:LocationBasedService rdf:type owl:Class ;
                      rdfs:subClassOf <http://www.w3.org/ns/ssn/System> ;
                      rdfs:comment "A location based service (LBS) is a service that provides the location of a person or object. It provides this information without the required knowledge of the underlying technologies and algorithms."@en ;
                      rdfs:isDefinedBy "https://isotc211.geolexica.org/concepts/278/"^^xsd:anyURI ;
                      rdfs:label "Location-based service"@en .


###  http://purl.org/poso/LowLevelFusion
:LowLevelFusion rdf:type owl:Class ;
                rdfs:subClassOf :SensorFusion ;
                rdfs:comment "Low Level Sensor Fusion is about fusing the raw data coming from multiple sensors. For example, we fuse point clouds coming from LiDARs and pixels coming from cameras."@en ;
                rdfs:isDefinedBy "https://www.thinkautonomous.ai/blog/?p=9-types-of-sensor-fusion-algorithms"^^xsd:anyURI ;
                rdfs:label "Low level sensor fusion"@en .


###  http://purl.org/poso/MagneticOdometry
:MagneticOdometry rdf:type owl:Class ;
                  rdfs:subClassOf :Odometry ;
                  rdfs:comment "Magnetic field odometry is the procedure of detecting movement by analyizing how the magnetic field is changing from one Observation to another."@en ;
                  rdfs:label "Magnetic odometry"@en .


###  http://purl.org/poso/MapOutput
:MapOutput rdf:type owl:Class ;
           rdfs:subClassOf <http://www.w3.org/ns/ssn/Output> ;
           rdfs:label "Map output"@en .


###  http://purl.org/poso/MidLevelFusion
:MidLevelFusion rdf:type owl:Class ;
                rdfs:subClassOf :SensorFusion ;
                rdfs:comment "Mid-Level sensor fusion is about fusing the objects detected independently on sensor data."@en ;
                rdfs:isDefinedBy "https://www.thinkautonomous.ai/blog/?p=9-types-of-sensor-fusion-algorithms"^^xsd:anyURI ;
                rdfs:label "Mid level sensor fusion"@en .


###  http://purl.org/poso/Motion
:Motion rdf:type owl:Class ;
        rdfs:subClassOf <http://www.w3.org/ns/ssn/Stimulus> ;
        rdfs:comment "Motion stimulus triggering an update of a position."@en ;
        rdfs:label "Beweging"@nl ,
                   "Motion"@en .


###  http://purl.org/poso/Multilateration
:Multilateration rdf:type owl:Class ;
                 rdfs:subClassOf :Lateration ;
                 rdfs:comment "Multilateration is the procedure of determining a position using relative distances to other known positions."@en ;
                 rdfs:label "Multilateration"@en ;
                 skos:altLabel "Hyperbolic positioning"@en .


###  http://purl.org/poso/NormalizationProcedure
:NormalizationProcedure rdf:type owl:Class ;
                        rdfs:subClassOf :CalibrationProcedure ;
                        rdfs:comment "Normalization procedure is a calibration procedure to normalize data."@en ;
                        rdfs:label "Normalization procedure"@en .


###  http://purl.org/poso/Odometry
:Odometry rdf:type owl:Class ;
          rdfs:subClassOf :DeadReckoning ;
          rdfs:comment "Odometry is the Procedure of calculating the current position of a moving FeatureOfInterest by using its previous position and Sensor Observation's indicating its heading and velocity."@en ;
          rdfs:label "Odometry"@en .


###  http://purl.org/poso/OpticalPositioningSystem
:OpticalPositioningSystem rdf:type owl:Class ;
                          rdfs:subClassOf :PositioningSystem ;
                          rdfs:comment "An optical positioning system is a positioning system that determines the position of an object by means of the properties of light."@en ;
                          rdfs:isDefinedBy "https://isotc211.geolexica.org/concepts/320/"^^xsd:anyURI ;
                          rdfs:label "Optical positioning system"@en .


###  http://purl.org/poso/Orientation
:Orientation rdf:type owl:Class ;
             rdfs:subClassOf <http://www.w3.org/ns/sosa/ObservableProperty> ,
                             <http://www.w3.org/ns/sosa/Result> ;
             rdfs:comment "De orientatie van een object in 2D of 3D."@nl ,
                          "The orientation of a feature of interest in 2D or 3D space."@en ;
             rdfs:label "Orientatie"@nl ,
                        "Orientation"@en .


###  http://purl.org/poso/OrientationOutput
:OrientationOutput rdf:type owl:Class ;
                   rdfs:subClassOf <http://www.w3.org/ns/ssn/Output> ;
                   rdfs:label "Orientation output"@en .


###  http://purl.org/poso/OutdoorDeployment
:OutdoorDeployment rdf:type owl:Class ;
                   rdfs:subClassOf <http://www.w3.org/ns/ssn/Deployment> ;
                   rdfs:comment "Describes the deployment of a System in an outdoor environment."@en ;
                   rdfs:label "Outdoor deployment"@en .


###  http://purl.org/poso/OutdoorPositioningSystem
:OutdoorPositioningSystem rdf:type owl:Class ;
                          rdfs:subClassOf :PositioningSystem ;
                          rdfs:comment "An outdoor positioning system defines a system that is used to determine a position outside a building without specifying the underlying technology."@en ;
                          rdfs:label "Outdoor positioning system"@en .


###  http://purl.org/poso/PDR
:PDR rdf:type owl:Class ;
     rdfs:subClassOf :DeadReckoning ;
     rdfs:comment "Pedestrian dead reckoning (PDR) is a positioning technique where the object is assumed to be a pedestrian that is walking or running. Using this knowledge, the dead reckoning involves the detection of steps and the step length to more accurately predict the movement."@en ;
     rdfs:label "Pedestrian dead reckoning"@en .


###  http://purl.org/poso/PolygonalAccuracy
:PolygonalAccuracy rdf:type owl:Class ;
                   rdfs:subClassOf <http://www.w3.org/ns/ssn/systems/Accuracy> ;
                   rdfs:label "Polygonal accuracy"@en .


###  http://purl.org/poso/Position
:Position rdf:type owl:Class ;
          rdfs:subClassOf <http://www.w3.org/ns/sosa/ObservableProperty> ,
                          <http://www.w3.org/ns/sosa/Result> ;
          rdfs:comment "A position indicates where an entity is located."@en ;
          rdfs:label "Positie"@nl ,
                     "Position"@en .


###  http://purl.org/poso/PositionOutput
:PositionOutput rdf:type owl:Class ;
                rdfs:subClassOf <http://www.w3.org/ns/ssn/Output> ;
                rdfs:label "Position output"@en .


###  http://purl.org/poso/PositioningPlatform
:PositioningPlatform rdf:type owl:Class ;
                     rdfs:subClassOf <http://www.w3.org/ns/sosa/Platform> ;
                     rdfs:comment "A positioning platform is a framework, architecture or platform used to develop and host a positioning system."@en ;
                     rdfs:label "Positioning platform"@en .


###  http://purl.org/poso/PositioningSystem
:PositioningSystem rdf:type owl:Class ;
                   rdfs:subClassOf <http://www.w3.org/ns/ssn/System> ,
                                   [ rdf:type owl:Restriction ;
                                     owl:onProperty <http://www.w3.org/ns/ssn/hasDeployment> ;
                                     owl:minQualifiedCardinality "1"^^xsd:nonNegativeInteger ;
                                     owl:onClass <http://www.w3.org/ns/ssn/Deployment>
                                   ] ;
                   rdfs:comment "A positioning system is a system of instrumental and computational components for determining position."@en ;
                   rdfs:isDefinedBy "https://isotc211.geolexica.org/concepts/349/"^^xsd:anyURI ;
                   rdfs:label "Positioning system"@en .


###  http://purl.org/poso/PositioningTechnique
:PositioningTechnique rdf:type owl:Class ;
                      rdfs:subClassOf <http://www.w3.org/ns/sosa/Procedure> ;
                      rdfs:comment "A positioning technique is a procedure to sample sensor data to an output position."@en ;
                      rdfs:label "Positioning technique"@en .


###  http://purl.org/poso/Proximity
:Proximity rdf:type owl:Class ;
           rdfs:subClassOf <http://www.w3.org/ns/ssn/Stimulus> ;
           rdfs:comment "Stimulus whenever two Feature of Interests are within close proximity."@en ;
           rdfs:label "Proximity" ;
           skos:example "A Feature Of Interest can be within close proximity of another Feature Of Interest without movement whenever the other Feature moved wihin the proximity of the first Feature."@en .


###  http://purl.org/poso/QuaternionOrientation
:QuaternionOrientation rdf:type owl:Class ;
                       rdfs:subClassOf :Orientation ,
                                       [ rdf:type owl:Restriction ;
                                         owl:onProperty :scalar ;
                                         owl:maxCardinality "1"^^xsd:nonNegativeInteger
                                       ] ,
                                       [ rdf:type owl:Restriction ;
                                         owl:onProperty :xAxisValue ;
                                         owl:maxCardinality "1"^^xsd:nonNegativeInteger
                                       ] ,
                                       [ rdf:type owl:Restriction ;
                                         owl:onProperty :yAxisValue ;
                                         owl:maxCardinality "1"^^xsd:nonNegativeInteger
                                       ] ,
                                       [ rdf:type owl:Restriction ;
                                         owl:onProperty :zAxisValue ;
                                         owl:maxCardinality "1"^^xsd:nonNegativeInteger
                                       ] ;
                       rdfs:label "Quaternion orientation"@en .


###  http://purl.org/poso/RFLandmark
:RFLandmark rdf:type owl:Class ;
            rdfs:subClassOf :Landmark ;
            rdfs:comment "A radio frequency landmark is a transmitting landmark that can be observed by its transmitting signals."@en ;
            rdfs:label "RF landmark"@en ;
            skos:example "An RF landmark example is a Bluetooth beacon that sends out a signal. Receivers of this signal can use the known position of this landmark to determine their relative position."@en .


###  http://purl.org/poso/RadioFrequencyFingerprinting
:RadioFrequencyFingerprinting rdf:type owl:Class ;
                              rdfs:subClassOf :Fingerprinting ;
                              rdfs:comment "Radio frequency fingerprinting or RF fingerprinting is a technique where RF signals are used to create a unique fingerprint at a current location."@en ;
                              rdfs:label "RF fingerprinting"@en .


###  http://purl.org/poso/RadioPropagation
:RadioPropagation rdf:type owl:Class ;
                  rdfs:subClassOf <http://www.w3.org/ns/sosa/Procedure> ;
                  rdfs:comment "The radio propagation formulas cover the computation of the radio waves through a medium (e.g. air)."@en ;
                  rdfs:isDefinedBy "https://en.wikipedia.org/wiki/Radio_propagation"^^xsd:anyURI ;
                  rdfs:label "Radio propagation"@en .


###  http://purl.org/poso/RelativeAcceleration
:RelativeAcceleration rdf:type owl:Class ;
                      rdfs:subClassOf :RelativePosition ;
                      rdfs:comment "A relative acceleration is a quantitative acceleration relative to another feature of interest."@en ;
                      rdfs:label "Relative acceleration"@en .


###  http://purl.org/poso/RelativeAngle
:RelativeAngle rdf:type owl:Class ;
               rdfs:subClassOf :RelativePosition ;
               rdfs:comment "A relative angle is a quantitative angle relative to another feature of interest."@en ;
               rdfs:label "Relatieve hoek"@nl ,
                          "Relative angle"@en ;
               skos:example "An example of relative angle is the Angle of Arrival."@en .


###  http://purl.org/poso/RelativeDistance
:RelativeDistance rdf:type owl:Class ;
                  rdfs:subClassOf :RelativePosition ;
                  rdfs:comment "A relative distance is a quantitative distance relative to another feature of interest."@en ;
                  rdfs:label "Relatieve afstand"@nl ,
                             "Relative distance"@en .


###  http://purl.org/poso/RelativePosition
:RelativePosition rdf:type owl:Class ;
                  rdfs:subClassOf :Position ,
                                  [ rdf:type owl:Restriction ;
                                    owl:onProperty :isRelativeTo ;
                                    owl:maxQualifiedCardinality "1"^^xsd:nonNegativeInteger ;
                                    owl:onClass <http://www.w3.org/ns/sosa/FeatureOfInterest>
                                  ] ;
                  rdfs:comment "A relative position is a position of a feature of interest with respect to the positions of other objects that this position is relative to."@en ,
                               "Een relatieve positie is een positie van een punt, met respect tot de posities van andere objecten die relatief zijn."@nl ;
                  rdfs:isDefinedBy "https://isotc211.geolexica.org/concepts/377/"^^xsd:anyURI ;
                  rdfs:label "Relatieve positie"@nl ,
                             "Relative position"@en .


###  http://purl.org/poso/RelativeSignalStrength
:RelativeSignalStrength rdf:type owl:Class ;
                        rdfs:subClassOf :RelativePosition ;
                        rdfs:comment "A relative signal strength is a received signal strength transmitted by another (RF) feature of interest."@en ;
                        rdfs:label "Relatieve signaalsterkte"@nl ,
                                   "Relative signal strength"@en .


###  http://purl.org/poso/RelativeVelocity
:RelativeVelocity rdf:type owl:Class ;
                  rdfs:subClassOf :RelativePosition ;
                  rdfs:comment "A relative velocity is a quantitative velocity relative to another feature of interest."@en ;
                  rdfs:label "Relatieve snelheid"@nl ,
                             "Relative velocity"@en .


###  http://purl.org/poso/SLAM
:SLAM rdf:type owl:Class ;
      rdfs:subClassOf :PositioningTechnique ;
      rdfs:comment "Simultaneous localization and mapping (SLAM) is the computational problem of constructing or updating a map of an unknown environment while simultaneously keeping track of an agent's location within it."@en ;
      rdfs:isDefinedBy "https://dbpedia.org/page/Simultaneous_localization_and_mapping"^^xsd:anyURI ;
      rdfs:label "Simultaneous localisation and mapping"@en .


###  http://purl.org/poso/SRS
:SRS rdf:type owl:Class ;
     rdfs:subClassOf <http://www.w3.org/ns/ssn/systems/SystemProperty> ;
     rdfs:comment "An identifiable and observable spatial reference system that represents the System's ability to operate its primary purpose in a specified reference system."@en ;
     rdfs:label "Spatial Reference System"@en .


###  http://purl.org/poso/SatellitePositioningSystem
:SatellitePositioningSystem rdf:type owl:Class ;
                            rdfs:subClassOf :PositioningSystem ;
                            rdfs:comment "In this context, satellite positioning implies the use of radio signals transmitted from \"active\" artificial objects orbiting the Earth and received by \"passive\" instruments on or near the Earth's surface to determine position, velocity, and/or attitude of an object."@en ;
                            rdfs:isDefinedBy "https://isotc211.geolexica.org/concepts/392/"^^xsd:anyURI ;
                            rdfs:label "Satellite positioning system"@en .


###  http://purl.org/poso/SensorFusion
:SensorFusion rdf:type owl:Class ;
              rdfs:subClassOf <http://www.w3.org/ns/sosa/Procedure> ;
              rdfs:comment "Sensor fusion is a procedure where multiple sensor data is combined to obtain a more reliable or accurate result."@en ;
              rdfs:isDefinedBy "https://en.wikipedia.org/wiki/Sensor_fusion"^^xsd:anyURI ;
              rdfs:label "Sensor fusion"@en .


###  http://purl.org/poso/SensorInput
:SensorInput rdf:type owl:Class ;
             rdfs:subClassOf <http://www.w3.org/ns/ssn/Input> ;
             rdfs:comment "Sensor input is input data provided by a sosa:Sensor"@en ;
             rdfs:label "Sensor input"@en .


###  http://purl.org/poso/TrackedFeature
:TrackedFeature rdf:type owl:Class ;
                rdfs:subClassOf <http://www.opengis.net/ont/geosparql#SpatialObject> ,
                                <http://www.w3.org/ns/sosa/FeatureOfInterest> ,
                                [ rdf:type owl:Restriction ;
                                  owl:onProperty :hasPosition ;
                                  owl:minQualifiedCardinality "1"^^xsd:nonNegativeInteger ;
                                  owl:onClass :Position
                                ] ;
                rdfs:comment "A feature of interest that is being tracked by a positioning system. This is the feature for which a position is observed."@en ;
                rdfs:label "Tracked feature"@en ;
                skos:example "The phone of a person that is being tracked in an indoor positioning system is the tracked feature."@en .


###  http://purl.org/poso/Triangulation
:Triangulation rdf:type owl:Class ;
               rdfs:subClassOf :Angulation ;
               rdfs:comment "Triangulation is the procedure of determining a position using relative angles to a feature of interest with a known position."@en ;
               rdfs:label "Triangulation"@en ;
               skos:altLabel "Angle-based positioning"@en .


###  http://purl.org/poso/Trilateration
:Trilateration rdf:type owl:Class ;
               rdfs:subClassOf :Lateration ;
               rdfs:comment "Trilateration is a positioning technique that uses exactly three reference points in 2D and four reference points in 3D to determine a position."@en ;
               rdfs:label "Trilateration"@en .


###  http://purl.org/poso/VSLAM
:VSLAM rdf:type owl:Class ;
       rdfs:subClassOf :SLAM ;
       rdfs:comment "Visual simultaneous localisation and mapping (VSLAM) is a positioning techniques that uses visual imagery to map an environment. Positioning works by detecting features of interest in image frames and comparing how these features move from one frame to another."@en ;
       rdfs:label "Visual simultaneous localisation and mapping"@en .


###  http://purl.org/poso/Velocity
:Velocity rdf:type owl:Class ;
          rdfs:subClassOf <http://www.w3.org/ns/sosa/ObservableProperty> ,
                          <http://www.w3.org/ns/sosa/Result> ;
          <http://qudt.org/schema/qudt/hasQuantityKind> <http://qudt.org/vocab/quantitykind/Velocity> ;
          rdfs:comment "Linear or angular velocity of a feature."@en ;
          rdfs:label "Velocity"@en .


###  http://purl.org/poso/VirtualLandmark
:VirtualLandmark rdf:type owl:Class ;
                 rdfs:subClassOf :Landmark ;
                 rdfs:comment "A virtual landmark is a spatial landmark with a known absolute or relative position but which is not detectable by any sensors without additional context."@en ;
                 rdfs:label "Virtual landmark"@en ;
                 skos:example "An example of a virtual landmark is a marker at a specific location."@en ,
                              "Image features can be considered landmarks as they are used by odometry and VSLAM algorithms."@en .


###  http://purl.org/poso/VisualInput
:VisualInput rdf:type owl:Class ;
             rdfs:subClassOf :SensorInput ;
             rdfs:label "Visual input"@en .


###  http://purl.org/poso/VisualLandmark
:VisualLandmark rdf:type owl:Class ;
                rdfs:subClassOf :Landmark ;
                rdfs:comment "A visual landmark is a feature of interest that visually present in the space."@en ;
                rdfs:label "Visual landmark"@en .


###  http://purl.org/poso/VisualOdometry
:VisualOdometry rdf:type owl:Class ;
                rdfs:subClassOf :Odometry ;
                rdfs:comment "Visual odometry is the procedure of detecting movement by analyzing how visual features are moving from one Observation image frame to another."@en ;
                rdfs:label "Visual odometry"@en .


###  http://www.opengis.net/ont/geosparql#Geometry
<http://www.opengis.net/ont/geosparql#Geometry> rdf:type owl:Class .


###  http://www.opengis.net/ont/geosparql#SpatialObject
<http://www.opengis.net/ont/geosparql#SpatialObject> rdf:type owl:Class .


###  http://www.w3.org/2000/01/rdf-schema#Class
rdfs:Class rdf:type owl:Class .


###  http://www.w3.org/ns/sosa/FeatureOfInterest
<http://www.w3.org/ns/sosa/FeatureOfInterest> rdf:type owl:Class .


###  http://www.w3.org/ns/ssn/System
<http://www.w3.org/ns/ssn/System> rdf:type owl:Class .


#################################################################
#    Individuals
#################################################################

###  http://purl.org/poso/XYX
:XYX rdf:type owl:NamedIndividual ,
              :EulerOrder ;
     rdfs:comment "The Euler rotation order for proper Euler angles."@en ;
     rdfs:label "X-Y-X" .


###  http://purl.org/poso/XYZ
:XYZ rdf:type owl:NamedIndividual ,
              :EulerOrder ;
     rdfs:comment "The Euler rotation (Tait‚ÄìBryan) order of X-axis, Y-axis, Z-axis."@en ;
     rdfs:label "X-Y-Z" .


###  http://purl.org/poso/XZY
:XZY rdf:type owl:NamedIndividual ,
              :EulerOrder ;
     rdfs:comment "The Euler rotation (Tait‚ÄìBryan) order of X-axis, Y-axis, Z-axis."@en ;
     rdfs:label "X-Z-Y" .


###  http://purl.org/poso/YXZ
:YXZ rdf:type owl:NamedIndividual ,
              :EulerOrder ;
     rdfs:comment "The Euler rotation (Tait‚ÄìBryan) order of X-axis, Y-axis, Z-axis."@en ;
     rdfs:label "Y-X-Z" .


###  http://purl.org/poso/YZX
:YZX rdf:type owl:NamedIndividual ,
              :EulerOrder ;
     rdfs:comment "The Euler rotation (Tait‚ÄìBryan) order of X-axis, Y-axis, Z-axis."@en ;
     rdfs:label "Y-Z-X" .


###  http://purl.org/poso/YZY
:YZY rdf:type owl:NamedIndividual ,
              :EulerOrder ;
     rdfs:comment "The Euler rotation order for proper Euler angles."@en ;
     rdfs:label "Y-Z-Y" .


###  http://purl.org/poso/ZXY
:ZXY rdf:type owl:NamedIndividual ,
              :EulerOrder ;
     rdfs:comment "The Euler rotation (Tait‚ÄìBryan) order of X-axis, Y-axis, Z-axis."@en ;
     rdfs:label "Z-X-Y" .


###  http://purl.org/poso/ZXZ
:ZXZ rdf:type owl:NamedIndividual ,
              :EulerOrder ;
     rdfs:comment "The Euler rotation order for proper Euler angles."@en ;
     rdfs:label "Z-X-Z" .


###  http://purl.org/poso/ZYX
:ZYX rdf:type owl:NamedIndividual ,
              :EulerOrder ;
     rdfs:comment "The Euler rotation (Tait‚ÄìBryan) order of X-axis, Y-axis, Z-axis."@en ;
     rdfs:label "Z-Y-X" .


###  Generated by the OWL API (version 4.5.9.2019-02-01T07:24:44Z) https://github.com/owlcs/owlapi
